<exercise>
<!-- source latex = 'generalizing_euclids_lemma.tex' -->
<!-- converted on 26/11/2021 at 16:53 -->
<statement>
<p>
Let <m>a,b,d\in\mathbb Z</m> such that <m>d\mid ab</m>. Show that the integer, <m> \frac{d}{\gcd(a,d)} </m>, divides <m>b</m>.
</p>
</statement>
<hint>
<p>
Try modifying the proof of <xref ref="lem-euclid">Euclid's lemma</xref>.
</p>
</hint>
<answer>
<p>
<xref ref="lem-euclid"/> proves the statement in the special case that <m>\gcd(a,d)=1</m>. We'll try to modify the proof of that lemma.
Bézout's identity tells us that there are <m>x,y\in\mathbb Z</m> so that
<me> \gcd(a,d)=xa+yd. </me>
We can rewrite this as
<me> 1 = x\cdot \frac{a}{\gcd(a,d)}+y\cdot\frac{d}{\gcd(a,d)} </me>
since <m>\gcd(a,d)</m> divides both <m>a</m> and <m>d</m>.
Now multiplying the entire equation by <m>b</m>, we have
<me> b=  x\cdot \frac{ab}{\gcd(a,d)}+yb\cdot\frac{d}{\gcd(a,d)}. </me>
The last step is to use that <m>d\mid ab</m> in order to show that this equation implies that <m>d/\gcd(a,d)</m> divides <m>b</m>.
</p>

</answer>
<solution>
<proof><p>
Let <m>a,b,d\in\mathbb Z</m> such that <m>d\mid ab</m>.
By Bézout's lemma, there are some <m>x,y\in \mathbb Z</m> such that <m>\gcd(a,d)=xa+yd</m>. Multiplying the equation by <m>b</m>, we have <m>b\gcd(a,d)=xab+ydb</m>. Since <m>d\mid ab</m>, there is some <m>k\in \mathbb Z</m> so that <m>ab=kd</m>.
Hence
<me> b\gcd(a,d)=xab+ydb=xkd+ydb=d(xk+yb). </me>
Now <m>\gcd(a,d)\mid d</m>, and so there is some <m>\ell\in\mathbb Z</m> so that <m>\ell\gcd(a,d)= d</m>. But then
<me> b\gcd(a,d)=\ell\gcd(a,d)(xk+yb) </me>
and as <m>\gcd(a,d)\neq0</m>,
<me> b=\ell(xk+yb).</me>
Since <m>xk+yb\in\mathbb Z</m>, we have <m>\ell \mid b</m>. But <m>\ell=d/\gcd(a,d)</m>, and so <m>d/\gcd(a,d)</m> divides <m>b</m>, as required.
</p></proof>

</solution>
</exercise>
