<?xml version="1.0" encoding="UTF-8"?>

<pretext>

<docinfo>
    <macros>
      \require{cancel}

      \newcommand{\ds}{\displaystyle}
      \newcommand{\es}{ {\varnothing}}
  		\newcommand{\st}{ \;:\; }
  		\newcommand{\pow}[1]{ \mathcal{P}\left(#1\right) }
  		\newcommand{\set}[1]{ \left\{#1\right\} }
      \newcommand{\Mod}[1]{\;(\mathrm{mod}\; #1)}
      \newcommand{\rel}{\;R\;}
  		\newcommand{\nrel}{\;\cancel{R}\;}
      \renewcommand{\neg}{\sim}
      \renewcommand{\text}[1]{\mathsf{\mbox{#1}}}
      \DeclareMathOperator{\gcd}{gcd}
      \DeclareMathOperator{\lcm}{lcm}
    </macros>
    <rename element="proposition" xml:lang="en-US">Result</rename>
</docinfo>

<slideshow>
  <title>PLP - 33</title>
  <subtitle>Topic 33<mdash />Injections, surjections and bijections</subtitle>

  <frontmatter>
  <titlepage>
    <author>
      <personname>Demirba≈ü &amp; Rechnitzer</personname>
      
    </author>
  </titlepage>


</frontmatter>

<section>
  <title>Injections, surjections and bijections</title>

<slide><title>Injections <mdash /> different maps to different</title>
<definition>
  <statement>
    <p>
      Let <m>f:A \to B</m> be a function.
    </p>
    <p>
      The function <m>f</m> is <term>injective</term> when for all <m>a_1,a_2 \in A</m>
      <me>
        (a_1 \neq a_2) \implies f(a_1)\neq f(a_2)
      </me>
      Equivalently (by the contrapositive)
      <me>
        f(a_1) = f(a_2) \implies a_1 = a_2
      </me>
      <term>Injections</term> are also called <term>one-to-one</term> functions.
    </p>
  </statement>
</definition>
<p>
  Note: if <m>f</m> is injective then for every <m>b \in B, |f^{-1}(\set{b})| \leq 1</m>.
</p>
<p>
  This is consistent with <m>|A| \leq |B|</m>
</p>
</slide>

<slide><title>Injection example</title>
<proposition>
  <statement>
    <p>
      The function <m>f: \mathbb{R} \to \mathbb{R}</m> defined by <m>f(x)=7x-3</m> is injective
    </p>
  </statement>
</proposition>
<p>
  Use <m>f(a_1)=f(a_2) \implies a_1=a_2</m> to prove <mdash /> equalities easier than inequalities.
</p>
<proof>
  <p>
    Let <m>x,z \in \mathbb{R}</m> and assume that <m>f(x)=f(z)</m>. Then we know that
    <md>
      <mrow> 7x-3 \amp= 7z-3 </mrow>
      <mrow> 7x\amp=7z </mrow>
      <mrow> x\amp=z </mrow>
    </md>
    and hence the function is injective.
  </p>
</proof>

</slide>

<slide><title>Surjections <mdash /> everything is mapped to by something</title>
<definition>
  <statement>
    <p>
      Let <m>g:A \to B</m> be a function.
    </p>
    <p>
      The function <m>g</m> is <term>surjective</term> when
      <me>
        \forall b \in B, \exists a \in A \text{ s.t. } g(a)=b
      </me>
      <term>Surjections</term> are also called <term>onto</term> functions.
    </p>
  </statement>
</definition>
<p>
  Note: if <m>g</m> is surjective then for every <m>b \in B, |g^{-1}(\set{b})| \geq 1</m>.
</p>
<p>
  This is consistent with <m>|A| \geq |B|</m>
</p>
</slide>

<slide><title>Surjection example</title>
<proposition>
  <statement>
    <p>
      The function <m>f: \mathbb{R} \to \mathbb{R}</m> defined by <m>f(x)=7x-3</m> is surjective
    </p>
  </statement>
</proposition>
<p>
  Given <m>y \in \mathbb{R}</m>, we need to find <m>x\in \mathbb{R}</m> so that <m>f(x)=y</m>:
  <me>
    y=7x-3 \qquad \text{so} \qquad y+3=7x \qquad \text{so} \qquad x = \frac{y+3}{7}.
  </me>
</p>
<proof>
  <p>
    Let <m>y \in \mathbb{R}</m> and set <m>x = \frac{y+3}{7} \in \mathbb{R}</m>.
    Then
    <me>
      f(x) = 7x-3 = 7\cdot \frac{y+3}{7}-3 = y+3 -3 = y
    </me>
    as required. Hence the function is surjective.
  </p>
</proof>
</slide>

<slide><title>A non-example</title>
<proposition>
  <statement>
    <p>
      The function <m>f: \mathbb{R} \to \mathbb{R}</m> defined by <m>f(x)=x^2</m> is neither injective nor surjective.
    </p>
  </statement>
</proposition>
<p>
  <md>
    <mrow> \text{not injective } \amp \equiv \exists x_1,x_2 \in A \text{ s.t. } (x_1\neq x_2) \land (f(x_1)=f(x_2))</mrow>
    <mrow> \text{not surjective} \amp \equiv \exists b \in B \text{ s.t. } \forall a \in A, f(a) \neq b</mrow>
  </md>
</p>
<proof>
  <p>
    We prove each claim in turn.
    <ul>
      <li>
        <p>
          Now let <m>x=1,z=-1</m>. Then since <m>f(x)= 1 = f(z)</m>, the function is not an injection.
        </p>
      </li>
      <li>
        <p>Let <m>y = -1</m>. For any <m>x \in \mathbb{R}</m> we know <m>f(x)=x^2 \geq 0</m>, so there is no <m>x \in \mathbb{R}</m> so that <m>f(x)=y</m>. So <m>f</m> is not a surjection.
        </p>
      </li>
    </ul>
  </p>
</proof>

</slide>

<slide><title>Bijections <mdash /> injective and surjective</title>
<definition>
  <statement>
    <p>
      Let <m>h:A \to B</m> be a function. The function <m>h</m> is <term>bijective</term> when it is both injective and surjective.
    </p>
    <p>
      <term>Bijections</term> are also called <term>one-to-one correspondences</term>.
    </p>
  </statement>
</definition>
<p>
  Note: if <m>h</m> is bijective then
  <ul>
    <li>since <m>h</m> is injective we know that for every <m>b \in B, |h^{-1}(\set{b})| \leq 1</m></li>
    <li>since <m>h</m> is surjective we know that for every <m>b \in B, |h^{-1}(\set{b})| \geq 1</m></li>
  </ul>
  and so for every <m>b \in B, |h^{-1}(\set{b})|=1</m>.
</p>
<p>
   This is consistent with <m>|A| = |B|</m>
</p>
<p>
  From work above <m>f: \mathbb{R} \to \mathbb{R}</m> defined by <m>f(x)=7x-3</m> is bijective.
</p>

</slide>


<slide><title>Another <m>x^2</m> example</title>
<p>
  Consider the 4 functions
  <md>
  <mrow>f :\amp\mathbb{R} \to \mathbb{R} \amp f(x) = x^2</mrow>
  <mrow>g :\amp\mathbb{R} \to [0,\infty) \amp g(x) = x^2</mrow>
  <mrow>h :\amp [0,\infty) \to \mathbb{R} \amp g(x) = x^2</mrow>
  <mrow>\rho :\amp [0,\infty) \to [0,\infty) \amp \rho(x) = x^2</mrow>
  </md>
</p>
<p>
  Then
  <ul>
    <li><m>f</m> is neither injective nor surjective</li>
    <li><m>g</m> is surjective but not injective</li>
    <li><m>h</m> is injective but not surjective</li>
    <li><m>\rho</m> is both injective and surjective</li>
  </ul>
  Let's prove the last one carefully.
</p>
</slide>

<slide><title>Injective and surjective</title>
<blockquote>
  <p><m>\rho : [0,\infty) \to [0,\infty)</m> with <m>\rho(x) = x^2</m> is injective and surjective</p>
</blockquote>
<proof>
  <p>
    We prove each in turn.
    <ul>
      <li>Injection: Let <m>x,z \in [0,\infty)</m> with <m>\rho(x)=\rho(z)</m>. Then we know that <m>x^2=z^2</m> and hence <m>x = \pm z</m>. But since <m>x,z \geq 0</m> we must have <m>x=z</m> as required.
    </li>
    <li>Surjection: Let <m>y \geq 0</m> and then set <m>x = \sqrt{y}</m>. Since <m>y \geq 0</m>, we know that <m>x \in \mathbb{R}</m>. Then <m>\rho(x) = x^2 = (\sqrt{y})^2 = y</m>.
    </li>
    <!-- <li><p>Surjection (without square-root, but with Calculus-1). Let <m>y \geq 0</m>. Notice that <m>\rho(x)</m> is continuous, so we can use the IVT
    <ul>
      <li>If <m>y=0</m> then set <m>x=0</m> and then <m>\rho(0)=0</m> as required</li>
      <li>If <m>y>0</m> then set <m>q=y+1</m>, notice that <m>\rho(q)=y^2+2y+1</m>  and since <m>y>0</m>, we know that <m>\rho(q)>y</m>. Then by the IVT, there is <m>0 \lt x \lt y+1</m> so that <m>\rho(x)=y</m> as required.</li>
    </ul></p>
    </li> -->
    </ul>
  </p>
</proof>

</slide>

</section>

</slideshow>
</pretext>
