<?xml version="1.0" encoding="UTF-8"?>

<pretext>

<docinfo>
    <macros>
      \newcommand{\ds}{\displaystyle}
      \newcommand{\es}{ {\varnothing}}
  		\newcommand{\st}{ \;\text{s.t.}\; }
  		\newcommand{\pow}[1]{ \mathcal{P}\left(#1\right) }
  		\newcommand{\set}[1]{ \left\{#1\right\} }
      \renewcommand{\neg}{\sim}
      \renewcommand{\text}[1]{\mathsf{\mbox{#1}}}
      \DeclareMathOperator{\gcd}{gcd}
      \DeclareMathOperator{\lcm}{lcm}
    </macros>
    <rename element="proposition" xml:lang="en-US">Result</rename>
</docinfo>

<slideshow>
  <title>PLP - 20</title>
  <subtitle>Topic 20<mdash />More induction</subtitle>

  <frontmatter>
  <titlepage>
    <author>
      <personname>Demirba≈ü &amp; Rechnitzer</personname>
      
    </author>
  </titlepage>


</frontmatter>


<section>
  <title>More examples</title>

  <slide><title>An inequality</title>
  <proposition>
    <statement>
      <p>
        Let <m>x \gt -1</m>, then for all <m>n \in \mathbb{N}</m>, <m>(1+x)^n \geq 1+nx</m>
      </p>
    </statement>
  </proposition>
  <p>
    <term>Scratch work</term>
    <ul>
      <li>When <m>n=1</m> we have <m>(1+x) = 1+x</m>, so all good</li>
      <li><p>Assume that <m>(1+x)^k \geq (1+kx)</m>, so
        <md>
          <mrow> (1+x)^{k+1}\amp = (1+x)\cdot(1+x)^{k} </mrow>
          <mrow> \amp \geq (1+x)(1+kx) = 1+(k+1)x+kx^2 </mrow>
          <mrow>\amp \geq 1+(k+1)x \amp \text{ since }x^2\geq 0</mrow>
        </md>
      </p>
      </li>
    </ul>
    Where did we use <m>x \gt -1</m>?
  </p>

  </slide>

<slide><title>Write it up nicely</title>
<proof>
  <p>We proceed by induction. Assume that <m>x \gt -1</m>.
    <ul>
      <li>Base case: When <m>n=1</m> we have <m>(1+x)=(1+x)</m>, as required</li>
      <li><p>
        Inductive step: Assume that the result holds for <m>n=k</m>, so <m>(1+x)^k \geq (1+kx)</m>. Then
      <md>
        <mrow>(1+x)^{k+1} \amp \geq (1+x)(1+kx) \amp\text{since }1+x \gt 0 </mrow>
        <mrow> \amp=1+(k+1)x+kx^2 </mrow>
        <mrow> \amp\geq 1+(k+1)x \amp \text{since } kx^2 \geq 0</mrow>
      </md>
      and so the result holds for <m>n=k+1</m>
        </p>
      </li>
      By induction the result holds for all <m>n \in \mathbb{N}</m>.
    </ul>
  </p>
</proof>
</slide>

<slide><title>Another example</title>
<proposition>
  <statement>
    <p>
      For all <m>n \in \mathbb{N}</m>, <m>1+3+\cdots+(2n-1) = n^2</m>.
    </p>
  </statement>
</proposition>

<p>
  <term>Scratch work</term>
  <ul>
    <li>Base case: When <m>n=1</m> we have <m>(2-1)=1^2</m>.</li>
    <li>Inductive step: Assume <m>1+3+\cdots+(2k-1)=k^2</m> then
    <md>
      <mrow> 1+3+\cdots+(2k-1) + (2k+1) \amp = k^2+(2k+1) </mrow>
      <mrow> \amp = (k+1)^2 </mrow>
    </md>
    as required.
  </li>
  </ul>
</p>
<p>
  <term>Warning</term> do not think <q><em>add the next term</em></q>. It is <q><em><m>P(k)\implies P(k+1)</m></em></q>
</p>
</slide>

<slide><title>Write it up</title>
<proof>
  <p>
    We prove the result by induction.
    <ul>
      <li>Base case: when <m>n=1</m>, we have <m>(2-1)=1^2</m>, as required.</li>
      <li>Inductive step: assume that <m>1+3+\cdots+(2k-1) = k^2</m>, but then
      <me>
        1+3+\cdots+ (2k-1) + (2k+1)  = k^2+2k+1 = (k+1)^2
      </me>
      Hence the inductive step holds.
      </li>
    </ul>
    So by induction the result holds for all <m>n \in \mathbb{N}</m>.
  </p>
</proof>

<p>
  <term>Warning</term> inductive step is not <q><em>add the next term</em></q>. It is <q><em><m>P(k)\implies P(k+1)</m></em></q>
</p>

</slide>

</section>

</slideshow>
</pretext>
