<?xml version="1.0" encoding="UTF-8"?>

<pretext>

<docinfo>
    <macros>
      \require{cancel}

      \newcommand{\ds}{\displaystyle}
      \newcommand{\es}{ {\varnothing}}
  		\newcommand{\st}{ \;:\; }
  		\newcommand{\pow}[1]{ \mathcal{P}\left(#1\right) }
  		\newcommand{\set}[1]{ \left\{#1\right\} }
      \newcommand{\Mod}[1]{\;(\mathrm{mod}\; #1)}
      \newcommand{\rel}{\;R\;}
  		\newcommand{\nrel}{\;\cancel{R}\;}
      \renewcommand{\neg}{\sim}
      \renewcommand{\text}[1]{\mathsf{\mbox{#1}}}
      \DeclareMathOperator{\gcd}{gcd}
      \DeclareMathOperator{\lcm}{lcm}
    </macros>
    <rename element="proposition" xml:lang="en-US">Result</rename>
</docinfo>

<slideshow>
  <title>PLP - 35</title>
  <subtitle>Topic 35<mdash />Inverse functions</subtitle>

  <frontmatter>
  <titlepage>
    <author>
      <personname>Demirba≈ü &amp; Rechnitzer</personname>
      
    </author>
  </titlepage>

</frontmatter>

<section><title>Inverse functions</title>
<slide><title>Inverses and one-sided inverses</title>
<definition>
  <statement>
    <p>
      Let <m>f: A \to B</m> and <m>g: B \to A</m> be functions.
      <ul>
        <li>If <m>g \circ f = i_A</m> then we say that <m>g</m> is a <term>left-inverse</term> of <m>f</m>.</li>
        <li>Similarly, if <m>f \circ g = i_B</m> then we say that <m>g</m> is a <term>right-inverse</term> of <m>f</m>.</li>
        <li>If <m>g</m> is both a <term>left-inverse</term> and <term>right-inverse</term>, then we call it an <term>inverse</term> of <m>f</m>.</li>
      </ul>
    </p>
  </statement>
</definition>
<p>
  Note that one can prove that if <em>an</em> inverse exists, then it is <em>unqiue</em>.
</p>
<p>
  So we can say <em>the</em> inverse and denote it <m>f^{-1}</m>.
</p>
</slide>

<slide><title>Left- but not right-inverse</title>
<p>
  Consider the functions <m>f,g</m> defined below
</p>
<sidebyside width="50%">
  <image source="figures/function_drawing5.png"/>
</sidebyside>
<p>
  Notice that
  <m>g(f(1))=1</m> and <m>g(f(2))=2</m>
  so <m>g</m> is a <term>left-inverse</term> of <m>f</m>.
</p>
<p>
  Then <m>f(g(4))=4,  f(g(5))=5</m> but <m>f(g(6))=5 \neq 6</m>
  so <m>g</m> is not a <term>right-inverse</term> of <m>f</m>.
</p>
<p>
  The non-injectiveness of <m>g</m> is to blame.
</p>
<p>
  A similar example gives a <term>right-inverse</term> that is not a <term>left-inverse</term> (non-surjectiveness is to blame)
</p>

</slide>

<slide><title>Existence of one-sided inverses</title>
<lemma>
  <statement>
    <p>
      Let <m>f:A \to B</m> be a function. Then
      <ul>
        <li><m>f</m> has a <term>left-inverse</term> iff <m>f</m> is injective.</li>
        <li><m>f</m> has a <term>right-inverse</term> iff <m>f</m> is surjective.</li>
      </ul>
    </p>
  </statement>
</lemma>
<p>
  The proofs of these statements make very good exercises. We'll do the forward implications.
</p>
</slide>

<slide><title>One sided inverse</title>
<blockquote>
  <p>If <m>f</m> has a left-inverse then it is injective</p>
</blockquote>
<proof>
  <p>
    Assume that <m>f</m> has a left-inverse <m>g</m>, so that <m>g(f(x))=x</m>.
  </p>
  <p>
  Now let <m>a_1,a_2 \in A</m>  so that <m>f(a_1)=f(a_2)</m>. Then we know that <m>g(f(a_1))=g(f(a_2))</m>. But since <m>g</m> is a left-inverse, <m>a_1=g(f(a_1))=g(f(a_2))=a_2</m>. Thus <m>f</m> is injective.
  </p>
</proof>

<blockquote>
  <p>If <m>f</m> has a right-inverse then it is surjective</p>
</blockquote>
<proof>
  <p>
    Assume that <m>f</m> has a right-inverse <m>g</m>, so that <m>f(g(y))=y</m>.
  </p>
  <p>
    Let <m>b \in B</m> and set <m>a=g(b)</m>. Then <m>f(a)= f(g(b)) = b</m>, since <m>g</m> is a right-inverse. Thus <m>f</m> is surjective.
  </p>
</proof>

</slide>

<slide><title>Joining inverses</title>
<lemma>
  <statement>
    <p>
      Let <m>f:A \to B</m> have a left-inverse <m>g</m> and a right-inverse <m>h</m>. Then <m>g=h</m>.
    </p>
  </statement>
</lemma>
<proof>
  <p>
    Let <m>f,g</m> and <m>h</m> be as stated. Thus
    <m>g\circ f = i_A</m> and <m>f\circ h = i_B</m>.
    Then
    <md>
      <mrow> g \amp = g \circ i_B = g \circ (f \circ h) </mrow>
      <mrow> \amp = (g \circ f) \circ h \amp \text{assoc of compositions} </mrow>
      <mrow> \amp =  i_A \circ h = h</mrow>
    </md>
    as required.
  </p>
</proof>

</slide>

<slide><title>Existence of inverse</title>
<theorem>
  <statement>
    <p>
      Let <m>f:A \to B</m>. Then <m>f</m> has an inverse iff <m>f</m> is bijective. Further, that inverse, if it exists, is unique.
    </p>
  </statement>
</theorem>

<proof>
  <p>
    <ul>
      <li>
        Assume that <m>f</m> has an inverse <m>g</m>. Then <m>g</m> is both a left-inverse and a right-inverse. Lemma: since <m>f</m> has a left-inverse, <m>f</m> is injective, and then since <m>f</m> has a right-inverse, <m>f</m> is surjective. Hence <m>f</m> is bijective.</li>
      <li>Now assume that <m>f</m> is bijective. Lemma: since <m>f</m> is injective, it has a left inverse, and since <m>f</m> is surjective, it has a right inverse. Lemma: those one-sided inverses are the same function, <m>g</m>. Hence <m>g</m> is an inverse of <m>f</m>.</li>
      <li><p>
        Finally, assume that <m>g,h</m> are inverses of <m>f</m>, then
        <m>
          g = g \circ (f \circ h) = (g \circ f)\circ h = h
        </m>.
        Thus the inverse function is unique.
      </p>
    </li>
    </ul>
  </p>
</proof>
</slide>

<slide><title>Example</title>
<proposition>
  <statement>
    <p>
      The function <m>f: \mathbb{R} \to \mathbb{R}, f(x)=7x-3</m> is bijective and so has an inverse.
    </p>
  </statement>
</proposition>
<proof>
  <p>
      Previously we showed that <m>f</m> is injective and surjective, and so is bijective. Hence its inverse exists.
  </p>
</proof>
<p>
  In this case we can find the inverse explicitly:
  <m>f^{-1}: \mathbb{R} \to \mathbb{R}</m> defined by <m>f^{-1}(y) = \frac{y+3}{7}</m>
</p>
<p>
  Since the function is bijective, enough to prove this is a left-inverse
  <me>
    (f^{-1} \circ f)(x) = f^{-1}(7x-3) = \frac{(7x-3)+3}{7} = x
  </me>
  as required.
</p>
</slide>

</section>
</slideshow>
</pretext>
