<?xml version="1.0" encoding="UTF-8"?>

<pretext>

<docinfo>
    <macros>
      \newcommand{\ds}{\displaystyle}
      \newcommand{\es}{ {\varnothing}}
  		\newcommand{\st}{ \;\mid\; }
  		\newcommand{\pow}[1]{ \mathcal{P}\left(#1\right) }
  		\newcommand{\set}[1]{ \left\{#1\right\} }
      \renewcommand{\neg}{\sim}
      \renewcommand{\text}[1]{\mathsf{\mbox{#1}}}
      \DeclareMathOperator{\gcd}{gcd}
      \DeclareMathOperator{\lcm}{lcm}
      \newcommand{\Mod}[1]{\;(\mathrm{mod}\; #1)}
    </macros>
</docinfo>

<slideshow>
<title>PLP - 10</title>
<subtitle>Topic 10 <mdash />Logical equivalence</subtitle>

<frontmatter>
<titlepage>
  <author>
    <personname>Demirba≈ü &amp; Rechnitzer</personname>
    
  </author>
</titlepage>


</frontmatter>


<section>
  <title>Tautologies and logical equivalence</title>

<slide><title>Tautologies and contradictions</title>
<p>
  Statements that are always true turn out to be very useful.
</p>

<definition><title>Tautologies and contradictions</title>
<statement>
<p>A <term>tautology</term> is a statement that is always true</p>
<p>A <term>contradiction</term> is a statement that is always false.</p>
</statement>
</definition>
<p>
  The following are examples of tautologies
  <me>
    P \lor (\neg P) \qquad \qquad
    \neg (P \lor Q) \iff ((\neg P) \land (\neg Q))
  </me>
</p>
<p>
  The following are examples of contradictions
  <me>
    P \land (\neg P) \qquad \qquad
    (P\land Q) \land ( (\neg P) \lor (\neg Q) )
  </me>
</p>

</slide>

<slide><title>A very useful tautology</title>
<p>
  <ul>
    <li>The statements <m>P \lor Q</m> and <m>Q \lor P</m> have the same truth-tables.</li>
    <li>The are <em>not the same</em> but they are <em>equivalent</em></li>
    <li>
      <p>
        We can express this by saying
        <q><em><m>(P \lor Q) \iff (Q \lor P)</m> is a tautology</em></q>
      </p>
    </li>
  </ul>
</p>

<definition>
<statement><p>
  Two statements <m>R</m> and <m>S</m> are <term>logically equivalent</term> when <q><m>R\iff S</m></q> is a tautology.
</p>
<p>In this case we write <m>R \equiv S</m>.</p>
</statement>
</definition>

<p>
  Showing logical equivalence
  <ul>
    <li>build the truth tables, or</li>
    <li>think about when each side is true and false</li>
  </ul>
</p>
</slide>

<slide>
  <title>A useful equivalence</title>
<p>
  Consider <m>(P \implies Q) \equiv (\neg P) \lor Q</m>.
</p>
<p>
  Why are these equivalent <mdash /> when true, when false?
  <ul>
    <li><em>Know your truth-tables!</em></li>
    <li>
      <term>LHS</term> is false only when <m>(P,Q)</m> = (T,F). Otherwise true.
    </li>
    <li>
      <term>RHS</term> is false when both <m>(\neg P), Q</m> are false, that is <m>(P,Q)</m> = (T,F). Otherwise false.
    </li>
  </ul>
  True at same time, false at same time. So equivalent.
</p>
<p>
  Can also build the truth-tables <mdash /> tedious but works.
</p>
<sidebyside>
  <tabular>
    <row>
    <cell><m>P</m> </cell>
    <cell><m>Q</m></cell>
    <cell><m>P \implies Q</m></cell>
    <cell><m>(\neg P) \lor Q</m></cell>
    </row>
    <row>
      <cell>T</cell>
      <cell>T</cell>
      <cell>T</cell>
      <cell>T</cell>
    </row>
    <row>
      <cell>T</cell>
      <cell>F</cell>
      <cell>F</cell>
      <cell>F</cell>
    </row>
    <row>
      <cell>F</cell>
      <cell>T</cell>
      <cell>T</cell>
      <cell>T</cell>
    </row>
    <row>
      <cell>F</cell>
      <cell>F</cell>
      <cell>T</cell>
      <cell>T</cell>
    </row>
  </tabular>
</sidebyside>

</slide>

<slide><title>Useful logical equivalences</title>
<theorem><title>Logical equivalences</title>
<statement><p>
  Let <m>P</m> and <m>Q</m> be statements. Then
<dl>
<li><title>Implication</title><p> <m>(P \implies Q) \equiv ( (\neg P)\lor Q) )</m></p></li>
<li><title>Contrapositive</title> <m>(P\implies Q) \equiv ((\neg Q) \implies (\neg P))</m></li>
<li><title>Biconditional</title><m>(P \iff Q) \equiv ( (P\implies Q) \land (Q\implies P))</m></li>
<li><title>Double negation</title> <m>\neg{(\neg{(P)})} \equiv P</m></li>
<li><title>Commutative laws</title><p>
<m>P \lor Q \equiv Q \lor P \qquad</m> and
<m>\qquad P \land Q \equiv Q \land P</m></p>
</li>
</dl>
</p></statement>
</theorem>

</slide>

<slide><title>Useful logical equivalences 2</title>
<theorem xml:id="thm-logical-equiv"><title>Logical equivalences</title>
<statement><p>
  Let <m>P, Q</m> and <m>R</m> be statements. Then
<dl>
<li><title>Associative laws</title><p>
 <m>P \lor (Q\lor R) \equiv (P \lor Q)\lor R \qquad</m>
and
 <m>\qquad P \land (Q\land R) \equiv (P \land Q)\land R</m></p>
</li>
<li><title>Distributive laws</title>
<p><m>P \lor (Q \land R) \equiv (P \lor Q) \land (P \lor R)\qquad </m>
and  <m>\qquad P \land (Q \lor R) \equiv (P \land Q) \lor (P \land R)</m></p>
</li>
<li><title>DeMorgan's laws</title>
<p><m>\neg{(P \lor Q)} \equiv (\neg{P}) \land (\neg{Q})\qquad </m>
and
<m>\qquad \neg{(P \land Q)} \equiv (\neg{P}) \lor (\neg{Q})</m>
</p></li>
</dl>
</p></statement>
</theorem>

</slide>

<slide><title>Back to the contrapositive</title>
<p>
  Show that <m>(P \implies Q) \equiv (\neg Q \implies \neg P)</m> using equivalences
  <md>
    <mrow> (P \implies Q) \amp \equiv (\neg P \lor Q) \amp \text{implication as or} </mrow>
    <mrow> \amp\equiv (Q \lor \neg P) \amp \text{commutes} </mrow>
    <mrow> \amp \equiv (\neg \neg Q \lor \neg P) \amp \text{double negative} </mrow>
    <mrow> \amp \equiv (\neg Q \implies \neg P) \amp \text{or as implication} </mrow>
  </md>
</p>

<p>
  Why is this useful a useful equivalence?
  <ul>
    <li>Contrapositive is <em>equivalent</em> to the original implication</li>
    <li>Proving one is true is <em>equivalent</em> as proving the other is true</li>
    <li>Sometimes the contrapositive is <em>easier</em> to prove than the original</li>
  </ul>
</p>
</slide>
</section>

</slideshow>
</pretext>
