<exercise>
<!-- source latex = 'sqrt_6_irrational.tex' -->
<!-- converted on 07/12/2021 at 12:25 -->
<statement>
<p>
Two irrationality proofs.
<ol marker="(a)">
<li>
<p>
 Prove that <m>\sqrt{6}</m> is an irrational number.
  </p></li>
<li>
<p>
 Prove that <m>\sqrt{2} + \sqrt{3}</m> is irrational.
</p>
</li>
</ol>
</p>
</statement>
<hint>
<p>
<ol marker="(a)">
<li>
<p>
 Remember that <m>2 \mid 6</m>.
  </p></li>
<li>
<p>
 The result from (a) can help you with (b). How can we manipulate <m>(\sqrt{2}+\sqrt{3})</m> to somehow get an expression involving <m>\sqrt{6}</m>? Or, alternatively, how can we use that expression to say something about <m>\sqrt{2}</m>?
</p>
</li>
</ol>
</p>
</hint>
<solution>

  <proof><title>Proof of (a)</title>
  <p>
  Assume, to the contrary that <m>\sqrt{6}</m> is rational. Then we can write <m>\sqrt{6} = \frac{a}{b}</m> with <m>a \in \mathbb{Z}, b \in \mathbb{N}</m> and <m>\gcd(a,b)=1</m>. Squaring both sides gives us <m> 6 = \frac{a^2}{b^2} </m> and so <m>a^2 =  6b^2</m>. Thus <m>6 \mid a^2</m>. This means that <m>a^2</m> is even, and so <m>a</m> is even.
</p>
<p>
  Since <m>a</m> is even we can write <m>a=2k</m> for some <m>k \in \mathbb{Z}</m>. But then
  <me>
    a^2 =4k^2 = 6b^2
  </me>
  This implies that <m>2k^2 = 3b^2</m>. This, in turn, implies that <m>3b^2</m> is even, since <m>3</m> is odd, we must have that <m>b^2</m> is even and so <m>b</m> is even. Now we have a contradiction since <m>2</m> divides both <m>a</m> and <m>b</m> but we assumed that <m>\gcd(a,b)=1</m>.
</p>
<p>
  Hence <m>\sqrt{6}</m> is irrational.
</p></proof>

<p>
Notice that we did not actually need, as part of the contradiction, to show that <m>6 \mid a \implies 6 \mid b</m>. We only needed that <m>\gcd(a,b) \neq 1</m> and it was sufficient to show that both were even.
</p>

<p>
 We give two proofs of (b).
</p>

<proof><title>First proof of (b)</title><p>
  Assume, to the contrary that <m>\sqrt{2}+\sqrt{3}</m> is rational. Then we can write
<me>
  \sqrt{2} + \sqrt{3} = \frac{a}{b}
</me>
where <m>a \in \mathbb{Z}, b\in\mathbb{N}</m> and <m>\gcd(a,b)=1</m>. Squaring both sides of this gives
<md>
<mrow>
  \frac{a^2}{b^2}  \amp = \left( \sqrt{2} + \sqrt{3} \right)^2
</mrow><mrow>
   \amp = 2 + 2\sqrt{2}\cdot\sqrt{3} + 3
</mrow><mrow>
   \amp = 5 + 2 \sqrt{6}
</mrow>
</md>
Rearranging this further, to isolate <m>\sqrt{6}</m>, gives
<md>
<mrow>
  2\sqrt{6}  \amp  = \frac{a^2}{b^2} - 5
</mrow><mrow>
  \sqrt{6}  \amp = \frac{a^2-5b^2}{2b^2}
</mrow>
</md>
which implies that <m>\sqrt{6} \in \mathbb{Q}</m>. This contradicts our result from (a). Thus it follows that <m>\sqrt{2}+\sqrt{3} </m> is irrational as required.
</p></proof>


<proof><title>Second proof of (b)</title><p>
  Assume, to the contrary, that <m> \sqrt{2}+\sqrt{3} </m> is rational. Hence we can write <m>\sqrt{2}+\sqrt{3} = \frac{a}{b}</m> with <m>a\in\mathbb{Z}, b\in \mathbb{N}</m>.
  But now rearrange this as
  <me>
  \sqrt{3} = \frac{a}{b} - \sqrt{2}.
  </me>
  Square both sides to get
  <me>
    3 = \frac{a^2}{b^2} - \frac{2a}{b} \sqrt{2} + 2
  </me>
  Now isolate <m>\sqrt{2}</m>:
  <md>
<mrow>
  \frac{2a}{b} \sqrt{2}  \amp = \frac{a^2}{b^2} -1  = \frac{a^2-b^2}{b^2}
</mrow><mrow>
  \sqrt{2}  \amp = \frac{a^2-b^2}{2ab}
  </mrow>
</md>
  This contradicts the fact that <m>\sqrt{2}</m> is irrational. Thus <m>\sqrt{2}+\sqrt{3}</m> is irrational.
</p>
<p>
  Notice that our manipulations require that <m>a \neq 0</m>, but since <m>\sqrt{2}+\sqrt{3} \neq 0</m>, this is easily verified.
</p></proof>

</solution>
</exercise>
