<exercise xml:id="ex_comp_inc_decr">
  <!-- source latex = 'Composition of increasing and decreasing functions.tex' -->
<!-- converted on 19/11/2021 at 11:20 -->
<statement>
<p>
We say that a function <m>f:\mathbb{R}\to \mathbb{R}</m> is <em>strictly increasing</em> if whenever <m>x_1  \lt  x_2</m> we have <m>f(x_1)  \lt  f(x_2)</m>. Similarly, a function <m>g: \mathbb{R}\to \mathbb{R}</m> is <em>strictly decreasing</em> if whenever <m>x_1  \lt  x_2</m> we have <m>g(x_1)  \gt  g(x_2)</m>.
<ol marker="(a)">
<li>
<p>
  Prove that the composition of two strictly increasing functions is strictly increasing.
    </p></li>
<li>
<p>
 Prove that the composition of two strictly decreasing functions is strictly increasing.
</p>
</li>
</ol>
</p>
</statement>

<!-- <hint></hint> -->

<solution>

  <proof><title>Proof of (a)</title>
  <p>
    Let <m>f,g:\mathbb{R}\to \mathbb{R}</m> be two strictly increasing functions. Fix <m>x_1, x_2 \in \mathbb{R}</m> with <m>x_1 \lt  x_2</m>. Then because <m>g</m> is strictly increasing,
    <me>z_1=g(x_1) \lt  g(x_2)=z_2.</me>
    Now, using the fact that <m>f</m> is strictly increasing and that <m>z_1\lt z_2</m>, we see that
    <me>(f\circ g)(x_1) = f(g(x_1)) = f(z_1)  \lt  f(z_2) = f(g(x_2)) = (f\circ g)(x_2).</me>
    Therefore <m>f\circ g</m> is a strictly increasing function.
  </p>
  </proof>

  <proof><title>Proof of (b)</title>
  <p>
    Let <m>f,g:\mathbb{R}\to \mathbb{R}</m> be two strictly decreasing functions. Fix <m>x_1, x_2 \in \mathbb{R}</m> with <m>x_1  \lt  x_2</m>. Then because <m>g</m> is strictly decreasing,
    <me>z_1 = g(x_1)  \gt  g(x_2)= z_2.</me>
    Now, using the fact that <m>f</m> is strictly decreasing and <m>z_2 \lt z_1</m>, we see that
    <me>(f\circ g)(x_2) = f(g(x_2)) = f(z_2)  \gt  f(z_1) = f(g(x_1)) = (f\circ g)(x_1)</me>
    Therefore <m>f\circ g</m> is a strictly increasing function.
  </p>
  </proof>
</solution>
</exercise>
