<exercise>
<!-- source latex = 'composition with injection and surjection.tex' -->
<!-- converted on 27/11/2021 at 15:24 -->
<statement>
<p>
Let <m>A, B</m> be nonempty sets. Let <m>f, h</m> be functions from <m>A</m> to <m>B</m>, and let <m>g</m> be a function from <m>B</m> to <m>A</m>.
</p>
<p>
<ol marker="(a)">
<li>
<p>
 Suppose that <m>g</m> is injective. Prove that if <m>g\circ f=g\circ h</m>, then <m>f=h</m>.
</p>
</li>
<li>
<p>
 Suppose that <m>g</m> is surjective. Prove that if <m>f \circ g=h\circ g</m>, then <m>f=h</m>.
</p>
</li>
</ol>
</p>
</statement>
<hint>
<p>
Two functions are equal when they are equal at all points in their domains.
</p>
</hint>
<solution>

  <proof><title>Proof of (a)</title>
  <p>
    Assume that <m>g</m> is injective and <m>g\circ f=g\circ h</m>. Then, we know that <m>\forall x\in A</m> we have <m>g\circ f(x)=g\circ h(x)</m>. Since <m>f(x), h(x)\in B</m>, we have, by the definition of function composition, <m>g( f(x))=g( h(x))</m>. Moreover, since <m>g</m> is injective, we conclude <m> f(x)= h(x)</m>. Since this is true for all <m>x\in A</m>, we conclude that  <m>f=h</m>.
    </p></proof>

  <proof><title>Proof of (b)</title>
  <p>
    Assume that <m>g</m> is surjective and  <m>f\circ g=h\circ g</m>. Let <m>x\in A</m>. Since <m>g</m> is a surjective function, we see that <m>\exists y\in B</m> such that <m>g(y)=x</m>. Hence, <m>f\circ g(y)=h\circ g(y)</m>. This implies <m>f(x) = f(g(y)) = h(g(y)) = h(x)</m>. Since this is true for all <m>x\in A</m>, we conclude that  <m>f=h</m>.
    </p></proof>

</solution>
</exercise>
