<exercise>
<!-- source latex = 'f compose g is g compose f .tex' -->
<!-- converted on 19/11/2021 at 11:28 -->
<statement>
<p>
Consider the following functions and their compositions.
<ol marker="(a)">
<li>
<p>
 Let <m>f:\mathbb{R}\to \mathbb{R}</m> be defined by <m>f(x)=x+1</m>. Does there exist a function <m>g:\mathbb{R}\to \mathbb{R}</m> such that <m>(f\circ g )(x) = (g\circ f)(x)</m> for every <m>x\in \mathbb{R}</m>?
    </p></li>
<li>
<p>
 Let <m>f:\mathbb{R}\to \mathbb{R}</m> be defined by <m>f(x)=c</m> for some <m>c\in \mathbb{R}</m> (i.e. <m>f</m> is a constant function). Which functions <m>g:\mathbb{R}\to \mathbb{R}</m> have the property <m>(f\circ g) (x) = (g\circ f)(x)</m> for every <m>x\in \mathbb{R}</m>?
    </p></li>
<li>
<p>
 Let <m>f:\mathbb{R}\to \mathbb{R}</m>. Suppose <m>(f\circ g)(x) = (g\circ f)(x)</m> for every <m>x\in \mathbb{R}</m> and for every function <m>g:\mathbb{R}\to \mathbb{R}</m>. Show that <m>f(x) = x</m>.
</p>
</li>
</ol>
</p>
</statement>
<hint>
<p>
Your observations from part (b) can be helpful in solving part (c).
</p>
</hint>
<solution>
<proof><title>Proof of (a)</title>
<p>  
<em>Claim:</em> There exists a suitable function <m>g</m>
</p>
 
<p>
  Consider <m>g(x)=x</m>. Then
  <me>(f \circ g )(x) = f(g(x)) = f(x) = x+1.</me>
  And on the other hand,
  <me>(g\circ f(x) )= g(f(x)) = g(x+1) = x+1.</me>
  Thus, <m>f\circ g = g\circ f</m>, as desired.
</p></proof>


<proof><title>Proof of (b)</title>
<p>
 <em>Claim:</em>  <m>g</m> can be any function such that <m>g(c)=c</m>.
</p>
<p>
    Notice that <m>(f\circ g)(x) = f(g(x))=c</m>, since <m>f</m> is a constant function. Then in order for <m>(f\circ g)(x) = (g \circ f)(x)</m> for every <m>x\in \mathbb{R},</m>
    <me>c= (g\circ f)(x) = g(f(x))=g(c).</me>
    Hence, we require that <m>g(c)=c</m>. There are no other conditions on the function <m>g</m>.
</p>
</proof>


<proof><title>Proof of (c)</title>
<p>
    Since the statement
    <me>(f\circ g)(x) = (g\circ f)(x) \tag{1}</me>
    must be true for any <m>x\in \mathbb{R}</m>, and any function <m>g:\mathbb{R}\to \mathbb{R}</m>, we begin by examining the restrictions placed on <m>f</m> when <m>g</m> is a constant function.
</p>
<p>
    Fix <m>c\in \mathbb{R}</m> and define the function <m>g_c:\mathbb{R}\to \mathbb{R}</m> by <m>g_c(x) = c</m>. By assumption, the statement <m>(f\circ g_c)(x) = (g_c\circ f)(x)</m> must hold. Applying part (b), we see that we must have <m>f(c)=c</m>.
</p>
<p>
    Moreover, since the choice of <m>c\in \mathbb{R}</m> was arbitrary and <m>(f\circ g_c)(x) = (g_c\circ f)(x)</m> must hold for every <m>c\in \mathbb{R}</m>, we know that <m>f(c)=c</m> for every <m>c\in \mathbb{R}</m>. This tells us that the function <m>f(x)=x</m> is the only function which could possibly satisfy (1).
</p>
<p>
    It remains to check that (1) holds for the function <m>f(x)=x</m>. Working with the left hand side, we see
    <me>(f\circ g)(x) = f(g(x)) = g(x)</me>
    Where <m>f(g(x)) = g(x)</m> by the definition of <m>f</m>. On the other hand,
    <me>(g\circ f)(x) = g(f(x)) = g(x)</me>
    Where we obtain the second equality using the fact that <m>f(x)=x</m>. Therefore,
    <me>(f\circ g)(x) = g(x) = (g\circ f)(x),</me>
    and we conclude that <m>f(x)=x</m> is the only solution to (1).
</p></proof>

</solution>
</exercise>
