<exercise>
<!-- source latex = 'f of f of f is bijective question.tex' -->
<!-- converted on 07/12/2021 at 12:07 -->
<statement>
<p>
The following question concerns the triple composition of a function.
<ol marker="(a)">
<li>
<p>
 Let <m>A</m> be a non-empty set and let <m>g:A \to A</m> be a function that satisfies <m>g\circ g\circ g=i_A</m>, where <m>i_A</m> is the identity function on the set <m>A</m>. Prove that <m>g</m> must be bijective.
</p>
</li>
<li>
<p>
 Let <m>A=\mathbb R -\{0,1\}</m> and let <m>f:A\to A</m> be defined by <m>f(x)=1-\frac{1}{x}</m>.  Show that <m>f\circ f\circ f = i_A</m> .
</p>
</li>
<li>
<p>
 Use part (a) to conclude that <m>f</m> is bijective and determine its inverse function <m>f^{-1}</m>.
</p>
</li>
</ol>
</p>
</statement>
<hint>
<p>
Make good use of the fact that
<me>
  g(g(g(x))) = (g \circ g)(  g(x) ) = i_A(x)= x.
</me>
</p>
</hint>

<!-- <answer> </answer> -->

<solution>

  <proof><title>Proof of (a)</title>
<p>
 Let <m>B</m> a set and assume that <m>g:A\to A</m> satisfies the condition <m>g\circ g\circ g=i_A</m>. We need to show that <m>g</m> is injective and surjective.
</p>
<p>
<ul>
<li>
<p>
 <em>Injective:</em> Let <m>x,y\in A</m> so that <m>g(x)=g(y)</m>. Since <m>g</m> is a function, this implies that <m>g( g(x) ) = g( g(y) )</m>. Applying <m>g</m> again gives <m>g( g( g(x) ) ) = g( g( g(y)))</m>, that is <m>(g \circ g \circ g)(x) = (g\circ g\circ g)(y)</m>. But, since <m>g\circ g\circ g=i_A</m>, the above implies that <m>i_A(x) = i_A(y)</m> and so <m>x=y</m>.
Therefore <m>g</m> is injective.
</p></li>
<li>
<p>
<em>Surjective</em>: Let <m>b\in A</m>. The,n since <m>g\circ g\circ g=i_A</m>, we get <m>g\circ g\circ g(b)=b</m>. Therefore, if we set <m>a = (g\circ g)(b) \in A</m>, we have <m>g(a)=b</m>. Hence, <m>g</m> is surjective.
</p></li>
</ul>
Therefore, we see that <m>g</m> is bijective.
</p>
  </proof>

 <proof><title>Proof of (b)</title>
<p>
 This requires some careful algebraic manipulations. Start by computing and simplifying <m>(f\circ f)(x)</m>
<md>
<mrow>
  f(f(x))  \amp = 1 - \dfrac{1}{1-\frac{1}{x}}
</mrow><mrow>
   \amp = 1 - \frac{x}{x-1} = \frac{x-1-x}{x-1}
</mrow><mrow>
   \amp  = \frac{-1}{x-1} = \frac{1}{1-x}
</mrow>
</md>
Then use this to compute <m> (f\circ f \circ f)(x)</m>:
<md>
<mrow>
  (f\circ f \circ f)(x) = f( (f\circ f)(x) )  \amp = 1 - \dfrac{1}{\frac{1}{x-1}}
</mrow><mrow>
   \amp = 1 - \frac{x-1}{1} = x
</mrow>
</md>
as required. Thus <m>f\circ f \circ f = i_A</m> as required.
</p>
 </proof>

<proof><title>Proof of (c)</title>
<p>
 The result from (a), implies that <m>f</m> is bijective. We can compute the inverse in two ways. First, observe that since  <m>f\circ f \circ f</m> is the identity
function, it follows that <m>\forall x\in A</m>, we have <m> (f \circ f)(x) =f^{-1}(x)= \frac{1}{1-x}</m> as calculated in part (b).
</p>
<p>
We could also solve for <m>f^{-1}</m> directly. Namely, if <m>f^{-1}(x)=y</m>, then we have
<md>
<mrow>
  x  \amp = f(y) = 1 - \frac{1}{y}
</mrow><mrow>
  xy  \amp = y-1
</mrow><mrow>
  xy-y  \amp = -1
</mrow>
</md>
from which we can conclude that
 <me> y = f^{-1}(x) = \frac{1}{1-x}.</me>
</p>
</proof>

</solution>
</exercise>
