<exercise>
<!-- source latex = '2eq1_proof.tex' -->
<!-- converted on 05/07/2021 at 19:55 -->
<statement>
<p>
Consider the faulty proof that <m>2=1</m>.
</p>

<proof><title>Faulty proof</title>
  <p>
Assume that <m>x=y</m>. Then multiplying both sides by <m>x</m> gives
<md>
<mrow>
    x^2  \amp = xy
</mrow><mrow>
    \Rightarrow x^2-y^2  \amp = xy - y^2
</mrow><mrow>
    \Rightarrow (x+y)(x-y)  \amp = y(x-y)
</mrow><mrow>
    \Rightarrow x+y  \amp = y
</mrow><mrow>
    \Rightarrow 2y  \amp = y
</mrow>
</md>
Letting <m>x=y=1</m>, we have shown that <m>2=1</m>.
</p></proof>

<p>
Identify any issues with the proof as written above.
</p>
</statement>
<solution>
<p>
First, this solution is quite terse, and it could benefit from more explanation. Explaining the steps taken in each line could make the error more clear:
</p>
<p>
Assume that <m>x=y</m>. Then
<md>
<mrow>
    x^2  \amp = xy  \amp \text{multiplying by } x
</mrow><mrow>
    \Rightarrow x^2-y^2  \amp = xy - y^2  \amp \text{Subtracting } y^2
</mrow><mrow>
    \Rightarrow (x+y)(x-y)  \amp = y(x-y)  \amp \text{Factoring}
</mrow><mrow>
    \Rightarrow x+y  \amp = y  \amp \text{Dividing by } (x-y)
</mrow><mrow>
    \Rightarrow 2y  \amp = y  \amp \text{Using } x=y
</mrow>
</md>
Letting <m>x=y=1</m>, we have shown that <m>2=1</m>.
</p>
<p>
The above proof is now more clear to read, and we notice that in the fourth line, we divide by <m>x-y</m>. We should always take care when we divide; we cannot divide by zero. Recall that we previously assumed that <m>x=y</m>, thus we are dividing by <m>0</m> in the fourth line. This is our logical error, and we can be reassured that <m>2\neq 1</m>.
</p>
<p>
In this proof, a careless division of an equation caused all the problems. Similar problems can arise when we work with inequalities. For example, multiplication or division of an inequality by a negative number will change the sign of the inequality, so we must take extra care to check if quantities are negative or not.
</p>
</solution>
</exercise>
