<exercise>
<!-- source latex = 'if n divides a and b it divides their linear combo.tex' -->
<!-- converted on 05/07/2021 at 13:20 -->
<statement>
<p>
Let <m>n,a,b,x,y\in\mathbb{Z}</m>. If <m>n\mid a</m> and <m>n\mid b</m>, then <m>n\mid (ax+by)</m>.
</p>
</statement>
<hint>
<p>
Think about what it means for <m>n</m> to divide <m>a</m> and <m>b</m>, and how we can use that information.
</p>
</hint>

<answer>
<p>
This may look slightly harder then the previous questions since it involves <m>5</m> different variables and a conjunction (an <q>and</q>) statement. But, since this is a conditional statement, our strategy is going to be the same. We are going to assume the hypothesis to be true and show the conclusion.
</p>
<p>
So, we assume that <m>n\mid a</m> and <m>n\mid b</m>. This means that <m>a=nk</m>, and <m>b=n\ell</m> for some <m>k,\ell\in\mathbb Z</m>. Once we have these expressions, we can bo back and try to see what we wanted to prove again.
</p>
<p>
We see that we want to prove that  <m>n\mid (ax+by)</m>. In other words, we want to prove <m>ax+by=nm</m> for some <m>m\in\mathbb Z</m>. Since we know that <m>a=nk</m>, and <m>b=n\ell</m>, we can write <m>ax+by=nkx+n\ell y=n(kx+\ell y)</m>. This is what we wanted to show. Let's write this in a nice proof.
</p>
</answer>

<solution>

<proof><p>
Assume <m>n,a,b,x,y\in\mathbb{Z}</m>, <m>n\mid a</m>, and <m>n\mid b</m>. This implies that <m>a=nk</m> and <m>b=n\ell</m> for some <m>k, \ell\in\mathbb{Z}</m>. Thus, <m>ax+by=nkx+n\ell y=n(kx+\ell y)</m>. Since <m>kx+\ell y\in\mathbb{Z}</m> for <m>k,x,\ell,y\in\mathbb{Z}</m>, then we see <m>n\mid (ax+by)</m>.
</p></proof>

</solution>
</exercise>
