<exercise xml:id="ex_sqrt_sum_ineq">
<!-- source latex = 'square_root_ineq.tex' -->
<!-- converted on 12/10/2021 at 12:29 -->
<statement>
<p>
Let <m>x,y\in\mathbb{R}</m> such that <m>x,y\geq0</m>. Show that <m>\sqrt{x+y}\leq \sqrt{x}+\sqrt{y}</m>.
</p>
<p>
You may use the following without proof:
</p>
<p>
<me> \text{If } 0\leq a\leq b, \text{ then } \sqrt{a}\leq \sqrt{b}. </me>
</p>
</statement>

<!-- <hint></hint> -->
<answer>
<p>
For scratchwork, we'll begin with the inequality
<me> \sqrt{x+y}\leq \sqrt{x}+\sqrt{y} </me>
Note that this is what we actually want to show though! When we write up the formal proof, we'll have to reverse the order of our logic.
We'll try to derive something true from this inequality, which will be the starting point of our actual proof.
Starting with
<me> \sqrt{x+y}\leq \sqrt{x}+\sqrt{y}, </me>
note that <m>0\leq \sqrt{x+y}</m>, and so we can square both sides to obtain
<me> x+y \leq x+2\sqrt{x}\sqrt{y}+y.</me>
Here we are using that <m>(\sqrt{x})^2=x</m> since <m>x\geq0</m>, and similarly for <m>y</m>.
Subtracting <m>x+y</m> from both sides of this inequality, we obtain
<me> 0 \leq \sqrt{x}\sqrt{y} </me>
and this inequality is true since the square root function is never negative.
So, for the actual proof of the statement, we should start with the inequality
<me> 0\leq\sqrt{x}\sqrt{y}, </me>
and reverse the argument above to show the desired conclusion,
<me> \sqrt{x+y}\leq \sqrt{x}+\sqrt{y}. </me>
</p>
</answer>

<solution>
<proof>
<p>
Let <m>x,y\in\mathbb{R}</m> such that <m>x,y\geq0</m>. Since the square root function is never negative,
<m>\sqrt{x}\sqrt{y}\geq0</m>. Then multiplying by <m>2</m> and adding <m>x+y</m> to both sides, we have
<me> x + y \leq x+2\sqrt{x}\sqrt{y}+y. </me>
Since <m>x,y\geq0</m>, we have that <m>(\sqrt{x})^2=x</m> and <m>(\sqrt{y})^2=y</m>, and so we may factor the righthand side of the above inequality to obtain
<me> x+y \leq (\sqrt{x}+\sqrt{y})^2. </me>
Since <m>x+y\geq0</m>, we then have
<me> \sqrt{x+y} \leq \sqrt{(\sqrt{x}+\sqrt{y})^2} </me>
But
<me> \sqrt{(\sqrt{x}+\sqrt{y})^2}=\sqrt{x}+\sqrt{y}, </me>
since <m>\sqrt{x}+\sqrt{y}\geq0</m>. Therefore
<me>\sqrt{x+y} \leq \sqrt{x}+\sqrt{y}, </me>
as required.
</p></proof>

</solution>
</exercise>
