<exercise>
<!-- source latex = 'Biconditional question where two divides n to the four minus seven.tex' -->
<!-- converted on 30/06/2021 at 14:02 -->
<statement>
<p>
Let <m>n\in\mathbb Z</m>. Show that <m>2\mid (n^4-7)</m> if and only if <m>4\mid (n^2+3)</m>.
</p>
</statement>
<hint>
<p>
Think carefully about the parity of <m>n</m>.
</p>
</hint>
<answer>
<p>
Since this is a biconditional statement, we need to prove the implication in both direction. That is we must prove
<md>
<mrow>
 \big(2\mid (n^4-7)\big)  \amp \implies \big(4\mid (n^2+3)\big).
  \amp  \text{and}  \amp  \amp
 \big(4\mid (n^2+3)\big)  \amp \implies  \big(2\mid (n^4-7)\big)
</mrow>
</md>
We'll prove each implication in turn.
</p>
</answer>
<solution>
<proof><p>
Let <m>n\in\mathbb{Z}</m>. We prove each implication in turn.
<ul>
<li>
<p>
  <m>(\Rightarrow)</m>: Assume that <m>2\mid (n^4-7)</m>. Then we see that <m>n^4-7=2k</m> for some <m>k\in\mathbb{Z}</m>. Thus, we see that <m>n^4=2(k+3)+1</m>. Since <m>(2k+3)\in\mathbb{Z}</m>, we see that <m>n^4</m> is odd. Since the square of an even number is even and <m>n^4=n^2n^2</m>, we see that <m>n^2</m> is odd. Similarly, we see that <m>n</m> is odd. Thus <m>n=2m+1</m> for some <m>m\in\mathbb{Z}</m>. Hence, <m>n^2+3=(4m^2+4m+1)+3=4(m^2+m+1)</m> and since <m>(m^2+m+1)\in\mathbb{Z}</m>, we see that <m>4\mid (n^2+3)</m>.
</p>
</li>
<li>
<p>
 <m>(\Leftarrow)</m>: Assume that <m>4\mid (n^2+3)</m>. Then we see that <m>n^2+3=4k</m> for some <m>k\in\mathbb{Z}</m>. Thus, we see that <m>n^2=2(2k-2)+1</m>. Since <m>(2k-2)\in\mathbb{Z}</m>, we see that <m>n^2</m> is odd. Moreover, since the product of two odd numbers is odd, we see that <m>n^4=n^2n^2</m> is odd. Thus <m>n^4=2m+1</m> for some <m>m\in\mathbb{Z}</m>. Hence, <m>n^4-7=2m-6=2(m-3)</m> and since <m>(m-3)\in\mathbb{Z}</m>, we see that <m>2\mid (n^4-7)</m>.
</p></li>
</ul>
Since both implications are true, the biconditional holds.
</p></proof>

</solution>
</exercise>
