<exercise>
<!-- source latex = 'transitivity_of_cardinality_leq.tex' -->
<!-- converted on 30/03/2022 at 15:36 -->
<statement>
<p>
Let <m>A</m>, <m>B</m>, and <m>C</m> be sets.
<ol marker="(a)">
<li>
<p>
 Suppose that <m>|A|\leq |B|</m> and <m>|B|\leq |C|</m>. Show that <m>|A|\leq |C|</m>.
</p></li>
<li>
  <blockquote>
<p>
 Show that the following statement is equivalent to the <xref ref="thm_CSB">Cantor-Schröeder-Bernstein</xref>:
</p>
  </blockquote>

<p>
Suppose that <m>|A|\leq |B|\leq |C|</m>, and that <m>|A|=|C|</m>. Then <m>|A|=|B|=|C|</m>.
</p>
</li>
</ol>
</p>
</statement>
<answer>
<p>
  <ol marker="(a)">
<li>
<p>
 By definition, we know that there is an injection from <m>A</m> to <m>B</m>, and from <m>B</m> to <m>C</m>. We need to use these to create an injection from <m>A</m> to <m>C</m>.
</p>
</li>
<li>
<p>
 We need to prove that the statement given in the question implies the Cantor-Schröeder-Bernstein Theorem,
and conversely, that the Cantor-Schröeder-Bernstein Theorem implies the given statement.
</p>
<p>
To prove the first implication, we assume that the statement given in the question is true; that is,
if <m>|A|\leq |B|\leq |C|</m> and <m>|A|=|C|</m>, then <m>|A|=|B|=|C|</m>. When we take <m>A=C</m>, we have the statement of the Cantor-Schroeder-Bernstein Theorem.
</p>
<p>
To prove the converse, we need to use the Cantor-Schröeder-Bernstein Theorem to establish the given statement:
</p>

<blockquote>
<p>
If <m>|A|\leq |B|\leq |C|</m> and <m>|A|=|C|</m>, then <m>|A|=|B|=|C|</m>.
</p>
</blockquote>

<p>
We'll try to prove that <m>|B|=|C|</m>. By <xref ref="thm_CSB"/>, we can do this by showing that <m>|B|\leq |C|</m> and <m>|C|\leq |B|</m>. The first is given by the statement of the problem. The second we will have to deduce from the assumption that <m>|A|=|C|</m>.
</p>
</li>
  </ol>
</p>
</answer>

<solution>
  <proof><title>Proof of (a)</title>
    <p>
Let <m>A</m>, <m>B</m> and <m>C</m> be sets such that <m>|A|\leq |B|</m> and <m>|B|\leq |C|</m>. Then, by definition, there are injections <m>f:A\rightarrow B</m> and <m>g:B\rightarrow C</m>.
By <xref ref="thm_comp_inj_surj"/>, the function <m>g\circ f:A\rightarrow C</m> is an injection. Thus, by definition, <m>|A|\leq |C|</m>.
</p></proof>


<proof><title>Proof of (b)</title>
<p>
First assume that whenever sets <m>A</m>, <m>B</m>, and <m>C</m> satisfy <m>|A|\leq |B|\leq |C|</m> and <m>|A|=|C|</m>, then we also have <m>|A|=|B|=|C|</m>.
Let <m>S</m> and <m>T</m> be set such that <m>|S|\leq |T|</m> and <m>|T|\leq |S|</m>.  Then applying the previous statement with <m>A=C=S</m> and <m>B=T</m>, we see that <m>|S|=|T|</m>.
This is precisely the statement of <xref ref="thm_CSB">Cantor-Schröeder-Bernstein</xref>.
</p>

<p>
Conversely, let <m>A</m>, <m>B</m> and <m>C</m> be sets such that <m>|A|\leq |B|</m> and <m>|B|\leq |C|</m>, and <m>|A|=|C|</m>.
Since <m>|A|=|C|</m>, there is a bijection, say <m>h</m>, from <m>C</m> to <m>A</m>. But <m>h</m> is also an injection, so <m>|C|\leq |A|</m>. Combining this with the inequality <m>|A|\leq |B|</m>, we have <m>|C|\leq |B|</m>, by part (a).
Therefore <m>|B|\leq |C|</m> and <m>|C|\leq |B|</m>, implying by <xref ref="thm_CSB">Cantor-Schröeder-Bernstein</xref> that <m>|B|=|C|</m>.
</p>

</proof>

</solution>
</exercise>
