<exercise>
<!-- source latex = 'Quantifier set question.tex' -->
<!-- converted on 24/06/2021 at 16:20 -->
<statement>
<p>
Given the sets,
<me>A=\set{n\in\mathbb Z\st 3\mid n}, B=\set{n\in\mathbb Z\st 4\nmid n}, \text{ and } C=\set{n\in\mathbb Z\st 6\nmid n}</me>
determine whether the following statements are true or false, and justify your answer.
</p>
<p>
<ol marker="(a)">
<li>
<p>
 <m>\forall a\in A</m>, <m>\exists b\in B</m> such that <m>a+b\in C</m>.
</p></li>
<li>
<p>
 <m>\exists a\in A</m> such that <m>\forall b\in B</m>, <m>a+b\in C</m>.
</p></li>
<li>
<p>
 <m>\forall a\in A</m>, <m>\forall b\in B</m>, <m>a+b\in C</m>.
</p></li>
<li>
<p>
 <m>\exists a\in A</m> and <m>\exists b\in B</m> such that <m>a+b\in C</m>.
</p>

</li>
</ol>
</p>
</statement>
<solution>
<p>
<ol marker="(a)">
<li>
<p>
 <m>\forall a\in A</m>, <m>\exists b\in B</m> such that <m>a+b\in C</m>.
</p>
<p>
This statement is true.
</p>
<p>
Let <m>a\in A</m>. Then we see that <m>a=3k</m> for some <m>k\in\mathbb{Z}</m>. Thus, since <m>k=2n</m> or <m>k=2n+1</m> for some <m>n\in\mathbb{Z}</m>, we see that <m>a=6n</m> or <m>a=6n+3</m> for some <m>n\in\mathbb{Z}</m>. Therefore if we pick <m>b=1\in B</m>, we get, <m>a+b=6n+1</m> or <m>a+b=6n+4</m>. Hence, <m>6\nmid (a+b)</m>.
</p>
</li>
<li>
<p>
 <m>\exists a\in A</m> such that <m>\forall b\in B</m>, <m>a+b\in C</m>.
</p>
<p>
This statement is false.
</p>
<p>
It helps to write out the negation: <m>\forall a \in A, \exists b\in B \text{ such that } a+b\notin C</m>. Let <m>a</m> be any element of <m>A</m>, then, as we saw in part (a), we know that <m>a=6n</m> or <m>a=6n+3</m> for some <m>n\in\mathbb{Z}</m>.
<ul>
<li>
<p>
 If <m>a=6n</m>, then we can pick <m>b=6\in B</m>, and we get <m>a+b=6n+6=6(n+1)</m>. Hence, <m>6\mid (a+b)</m>, that is, <m>(a+b)\notin C</m>.
</p></li>
<li>
<p>
  Similarly, if <m>a=6n+3</m>, we can pick <m>b=3\in B</m>, and get <m>a+b=6n+6=6(n+1)</m>. Hence,  <m>6\mid (a+b)</m>, that is, <m>(a+b)\notin C</m>.
</p></li>
</ul>
So in either case, we can pick <m>b \in B</m> so that <m>a+b \notin C</m>. Since  the negation is true, the original statement is false.
</p>
</li>
<li>
<p>
 <m>\forall a\in A</m>, <m>\forall b\in B</m>, <m>a+b\in C</m>.
</p>
<p>
This statement is false.
</p>
<p>
Again, it helps to write out the negation: <m>\exists a \in A \text{ such that } \exists b\in B\text{ such that } a+b \notin C </m>. So it suffices to find an example of <m>a,b</m> so that <m>a+b \notin C</m>. We can take <m>a=3\in A</m> and <m>b=3\in B</m>; and get <m>a+b=6</m>. This means <m>6\mid (a+b)</m>. Thus, <m>(a+b)\notin C</m>. Since the negation is true, the original statement is false.
</p>
</li>
<li>
<p>
 <m>\exists a\in A</m> and <m>\exists b\in B</m> such that <m>a+b\in C</m>.
</p>
<p>
This statement is true.
</p>
<p>
 Since both quantifiers are <q>there exists</q>, we only need an example. We can take <m>a=0\in A</m> and <m>b=1\in B</m>, and get <m>a+b=1</m> and hence, <m>6\nmid (a+b)</m>. Thus, <m>(a+b)\in C</m>.
</p>


</li>
</ol>
</p>
</solution>
</exercise>
