<exercise>
<!-- source latex = 'sequence limit.tex' -->
<!-- converted on 08/11/2021 at 10:38 -->
<statement>
<p>
Prove that
<me>\displaystyle \lim_{n\to\infty}\left(1-\frac{2}{n^2}-\frac{3}{n^3}\right)=1. </me>
</p>
<p>
You may use the following fact: Let <m>x,y</m> be positive real numbers. Then
<me>  \sqrt{x} \lt\sqrt{y} \iff x\lt y. </me>
</p>
</statement>

<!-- <hint></hint> -->

<answer>
<p>
Recall from the definition of a limit that the proof should go like this:
We're given some <m>\epsilon\gt 0</m>. We need to find some <m>N\in\mathbb{N}</m> so that whenever <m>n\gt N</m>, we have
<me> \left|1-\frac{2}{n^2}-\frac{3}{n^3}-1\right| \lt \epsilon. </me>
Let's unravel this inequality to see how large <m>n</m> needs to be. We want to rewrite this inequality so that's in the form <m>n</m> greater than <em>something</em>; this <em>something</em> will tell us how large we need to take <m>N</m> so that the inequality above is satisfied.
</p>
<p>
Now since,
<me>
\left|\left(1-\frac{2}{n^2}-\frac{3}{n^3}\right)-1\right| =
\left|-\frac{2}{n^2}-\frac{3}{n^3} \right| =  \frac{2}{n^2}+\frac{3}{n^3}
</me>
the inequality can be simplified to
<me> \frac{2}{n^2}+\frac{3}{n^3} \lt \epsilon. </me>
Because we have two different terms with <m>n</m> in them, it may be difficult to put the inequality in the form we'd like, that is, <m>n</m> greater than something.
What we can do instead is consider which of the factors <m>1/n^2</m> or <m>1/n^3</m> is larger - and then only working with the larger one, by bounding the smaller one by it.
</p>
<p>
Since <m>n \in \mathbb{N}</m> we know that <m>n \geq 1</m>. Dividing this inequality by <m>n^3</m> (which is positive), then gives us
<me>
  \frac{1}{n^2} \geq \frac{1}{n^3}
</me>
This means that
<me> \frac{2}{n^2}+\frac{3}{n^3} \leq \frac{2}{n^2}+\frac{3}{n^2} =\frac{5}{n^2}. </me>
Therefore, if we show that
<me> \frac{5}{n^2}\lt \epsilon, </me>
we'll also have that
<me> \frac{2}{n^2}+\frac{3}{n^3} \lt \epsilon. </me>
Now, we can take the square root of both sides of the inequality <m>5/n^2\lt\epsilon</m>, and use the reverse implication in the fact given in the question to say that
<me> \frac{\sqrt{5}}{\sqrt{\epsilon}}\lt n. </me>
We can actually reverse all of these steps (so we use the forward implication in the given fact), to get the following implication:
<me> \frac{\sqrt{5}}{\sqrt{\epsilon}}\lt n \implies \left|1-\frac{2}{n^2}-\frac{3}{n^3}-1\right| \lt \epsilon. </me>
This tells us that we can take <m>N</m> to be any natural number that is larger than <m>\sqrt{5}/\sqrt{\epsilon}</m>.
</p>
<p>
  So we can now write up the proof.
</p>


<p>
But we have actually missed an opportunity to simplify things further here. Recall that by dividing the inequality <m>n \geq 1</m> by <m>n^3</m> we showed that <m>\frac{1}{n^2} \geq \frac{1}{n^3}</m> and used that to simplify the inequalities that we needed for our proof.  We can simplify things further still by noting that by dividing the inequality <m>n \geq 1</m> by <m>n^2</m> we get
<me>
  \frac{1}{n} \geq \frac{1}{n^2}
</me>
So we can use that to show
<me> \frac{2}{n^2}+\frac{3}{n^3} \leq \frac{2}{n^2}+\frac{3}{n^2} =\frac{5}{n^2} \leq \frac{5}{n}.
</me>
Then it suffices to find <m>n</m> big enough so that
<me>
  \frac{5}{n} \leq \epsilon
</me>
which is quite a bit easier than the mucking around with square-roots we had to do before.
</p>

</answer>

<solution>
<proof><title>First proof</title>
<p>
Let <m>\epsilon \gt 0</m> be given. Let <m>N=\left\lceil \sqrt{\frac{5}{\epsilon}}\right\rceil</m>. Note this implies that <m>N^2\geq 5/\epsilon</m>.
Now suppose that <m>n\in\mathbb{N}</m>, <m>n\gt N</m>. Since <m>n=\sqrt{n^2}</m> and <m>N=\sqrt{N^2}</m> we can use the given fact to say that
<me> n^2\gt N^2\geq \frac{5}{\epsilon}, </me>
and so <m>5/n^2\lt \epsilon</m>. Moreover, since <m>n\geq 1</m>, we have <m>n^3\geq n^2</m>, and so <m>1/n^3\leq 1/n^2</m>.
Using these two inequalities, we therefore have
<me> \left|1-\frac{2}{n^2}-\frac{3}{n^3}-1\right| =\frac{2}{n^2}+\frac{3}{n^3}\leq\frac{5}{n^2}\lt\epsilon. </me>
And thus the sequence converges to 1 as required.
</p>
</proof>


<proof><title>Simpler proof</title>
  <p>
Let <m>\epsilon \gt 0</m> be given. Let <m>N=\left\lceil \frac{5}{\epsilon}\right\rceil</m>. Notice that when <m>n \geq N</m>, we have that
<me>
  \frac{5}{n} \lt \frac{5}{N} \leq \epsilon.
</me>
Since <m>n \geq 1</m>, we know that
<me>
\frac{1}{n} \gt \frac{1}{n^2} \geq \frac{1}{n^3}
</me>
Hence
<me> \left|1-\frac{2}{n^2}-\frac{3}{n^3}-1\right| =\frac{2}{n^2}+\frac{3}{n^3}\leq\frac{5}{n}\lt\epsilon. </me>
Thus the sequence converges to 1.
</p></proof>

<p>
We shouldn't feel bad that we made a more complicated proof first; It
is a normal part of doing mathematics. Our first proof of a result is
often <q>bettered</q> by our second proof.
</p>

</solution>
</exercise>
