<exercise>
<!-- source latex = 'sum_functions_odd.tex' -->
<!-- converted on 18/08/2021 at 14:52 -->
<statement>
<p>
Let <m>f:\mathbb{R}\to\mathbb{R}</m> be a function. We say that <m>f</m> is
<ul>
<li>
<p>
 even if <m>f(-x)=f(x)</m> for all <m>x\in\mathbb{R}</m>;
</p></li>
<li>
<p>
  odd if <m>f(-x)=-f(x)</m> for all <m>x\in\mathbb{R}</m>.
</p></li>
</ul>
</p>
<p>
Let <m>f:\mathbb{R}\to\mathbb{R}</m> and <m>g:\mathbb{R}\to\mathbb{R}</m>. If <m>f+g</m> is odd, are <m>f</m> and <m>g</m> also odd?
</p>
</statement>
<hint>
<p>
Try playing around with some simple functions.
</p>
</hint>
<answer>
<p>
We'll try to construct a pair of function <m>f,g</m> so that <m>f+g</m> is odd, but one of them, say <m>f</m>, is even.
We can test the result by look at some simple odd and even functions.
An example of an odd function is <m>y=x</m>, and an example of an even function is <m>y=x^2</m>.
Let's suppose that <m>f(x)=x^2</m>, which is even. We want to choose <m>g</m> so that <m>f+g=x</m>, an odd function. Then we can take <m>g(x)=x-f(x)=x-x^2</m>.
Also, we can show that <m>g</m> is neither even nor odd;  <m>g(2)=-2</m> but <m>g(-2)=-6</m>.
</p>
</answer>

<solution>
<proof>
<p>
Let <m>f:\mathbb{R}\to\mathbb{R}</m> be defined by <m>f(x)=x^2</m>, and let <m>g:\mathbb{R}\to\mathbb{R}</m> be defined by <m>g(x)=x-x^2</m>.
Then for any <m>x\in\mathbb{R}</m>,
<me> f(x)=x^2=(-x)^2=f(-x) </me>
so <m>f</m> is even, not odd. Moreover, <m>(f+g)(x)=x^2+(x-x^2)=x</m>. Then
<me> (f+g)(x)=x=-(f+g)(-x) </me>
and so <m>f+g</m> is odd. Therefore just because the sum of two functions is an odd function, it does not follow that those two functions are odd functions.
</p></proof>

</solution>
</exercise>
