<exercise>
<!-- source latex = 'log_equiv.tex' -->
<!-- converted on 18/08/2021 at 14:22 -->
<statement>
<p>
Show that the following pairs of statements are logically equivalent using <xref ref="thm-logical-equiv"/>.
</p>
<p>
<ol marker="(a)">
<li xml:id="prob-contrapos-bicond">
<p>
 <m>P\iff Q</m> and <m>(\neg P) \iff (\neg Q)</m>
</p></li>
<li>
<p>
 <m>P\implies(Q\lor R)</m> and <m>P\implies((\neg Q) \implies R)</m>
</p></li>
<li>
<p>
 <m>(P\lor Q)\implies R</m> and <m>(P\implies R)\land(Q\implies R)</m>
</p>
</li>
</ol>
</p>
</statement>

<!-- <hint></hint> -->

<solution>
<p>
<ol marker="(a)">
<li>
<p>
 Using the biconditional equivalence, we have
<me> (P\iff Q) \equiv ((P\implies Q)\land (Q\implies P)). </me>
Then using the contrapositive equivalence, we have
<me> ((P\implies Q)\land (Q\implies P)) \equiv  \big(((\neg Q)\implies (\neg P))\land ((\neg P)\implies (\neg Q))\big) </me>
and by commutativity, this is logically equivalent to
<me> ((\neg P)\implies (\neg Q)) \land ((\neg Q)\implies (\neg P)).</me>
Finally, by the biconditional equivalence, this is logically equivalent to
<me> (\neg P) \iff (\neg Q) </me>
</p>
</li>
<li>
<p>
 By the implication equivalence and the double negation equivalence, we have
<me> (P\implies(\neg Q\implies R))\equiv \big(P\implies((\neg(\neg Q))\lor R)\big)\equiv (P\implies(Q\lor R)). </me>
</p>
</li>
<li>
<p>
 By the implication equivalence and DeMorgan's law,
<me> ((P\lor Q)\implies R)\equiv ((\neg(P\lor Q))\lor R) \equiv \big(((\neg P)\land (\neg Q))\lor R\big). </me>
Then using commutativity and then the distribution law, this is logically equivalent to
<me> \big(R\lor ((\neg P)\land (\neg Q))\big)\equiv \big((R\lor (\neg P))\land (R\lor (\neg Q))\big) </me>
Then by commutativity and then the implication equivalence, this is logically equivalent to
<me> \big(((\neg P)\lor R)\land ((\neg Q) \lor R)\big) \equiv ((P\implies R)\land(Q\implies R)). </me>
</p>
</li>
</ol>
</p>
</solution>
</exercise>
