<exercise>
<!-- source latex = 'negate english statements using symbolic logic question_callback to a a question before.tex' -->
<!-- converted on 05/07/2021 at 10:52 -->
<statement>
<p>
Use the logical equivalences given in <xref ref="thm-logical-equiv"/> and <xref ref="thm-neg-imp"/> to negate the following sentences.
</p>
<p>
<ol marker="(a)">
<li>
<p>
 <m>8</m> is even and <m>5</m> is prime.
</p></li>
<li>
<p>
 If <m>n</m> is a multiple of <m>4</m> and <m>6</m>, then it is a multiple of <m>24</m>.
</p></li>
<li>
<p>
 If <m>n</m> is not a multiple of <m>10</m>, then it is a multiple of <m>2</m> but is not a multiple of <m>5</m>.
</p></li>
<li>
<p>
  <m>3\leq x\leq 6</m>.
</p></li>
<li>
<p>
 A real number <m>x</m> is less than <m>-2</m> or greater than <m>2</m> if its square is greater than <m>4</m>.
</p></li>
<li>
<p>
  If a function <m>f</m> is differentiable everywhere then whenever <m>x\in\mathbb{R}</m> is a local maximum of <m>f</m> we have <m>f'(x)=0</m>.
</p>
</li>
</ol>
</p>
</statement>
<hint>
<p>
Refer back to <xref ref="ex2-trans-eng-to-logic"/> and use <xref ref="thm-logical-equiv"/>.
</p>
</hint>
<solution>
<p>
In this question, first we are going to write the sentences in symbolic logic, then negate them using the <xref ref="thm-logical-equiv"/> and finally we will rewrite these negations in English.
</p>
<p>
<ol marker="(a)">
<li>
<p>
  This sentence can be written as <m>P\land Q</m> for
<md>
<mrow>
P: \amp \quad 8  \text{ is even}
</mrow><mrow>
Q: \amp \quad 5  \text{ is prime}.
</mrow>
</md>
So, its negation is:
<me>
{\neg} (P\land Q)\equiv ({\neg} P)\lor ({\neg} Q)
</me>
Here, we used DeMorgan's law. Then, the negation can be rewritten as:
<md>
<mrow>
  \text{8 is not even or 5 is not prime}.
</mrow>
</md>
</p>
</li>
<li>
<p>
   This sentence can be written as <m>(P\land Q)\implies R</m> for
<md>
<mrow>
P:  \amp \quad n \text{ is a multiple of } 4,
</mrow><mrow>
Q:  \amp \quad n \text{ is a multple of } 6,
</mrow><mrow>
R:  \amp \quad n \text{ is a multiple of } 24.
</mrow>
</md>
Then its negation is:
<me>
{\neg}\left( (P\land Q)\Rightarrow R\right)\equiv {\neg}\left( {\neg} (P\land Q) \lor R  \right)\equiv (P\land Q)\land {\neg} R.
</me>
Here, we used the equivalence of implication, DeMorgan's law and double negation. Then, the negation can be rewritten as:
<md>
<mrow>
n \text{ is a multiple of 4 and 6, but it is not a multiple of 24.}
</mrow>
</md>
</p>
</li>
<li>
<p>
 This sentence can be written as <m>(\neg P)\implies \big(Q\land (\neg R)\big)</m> for
<md>
<mrow>
P: \amp \quad n \text{ is a multiple of } 10,
</mrow><mrow>
Q: \amp \quad n \text{ is a multiple of } 2,
</mrow><mrow>
R: \amp \quad n \text{ is a multiple of } 5.
</mrow>
</md>
</p>
<p>
Then, we see that the negation is:
<md>
<mrow>
\neg\!\left(\neg P\implies \big(Q\land (\neg R)\big)\right) \amp \equiv\ \neg\!\left(\neg(\neg P)\lor \big(Q\land(\neg R)\big)\right)
</mrow><mrow>
 \amp \equiv (\neg P)\land \neg\big(Q\land (\neg R)\big)
</mrow><mrow>
 \amp \equiv (\neg P)\land \big((\neg Q) \lor R\big)
</mrow><mrow>
 \amp \equiv \big((\neg P)\land (\neg Q)\big)\lor \big( (\neg P)\land R \big).
</mrow>
</md>
Here, first we used the equivalence of implication. Then DeMorgan's law and double negation, and finally distribution law. This means that we can rewrite the negation as:
<md>
<mrow>
 \amp n \text{ is not a multiple of 10 and } n  \text{ is not a multiple of 2, or }
</mrow><mrow>
 \amp n  \text{ is not a multiple of 10 and } n \text{ is a multiple of 5.}
</mrow>
</md>
</p>
</li>
<li>
<p>
  This expression can be written as <m>P\land Q</m> for
<md>
<mrow>
P: \amp  \quad x \geq 3,
</mrow><mrow>
Q: \amp  \quad x\leq 6.
</mrow>
</md>
Then its negation is:
<me>
{\neg} (P\land Q)\equiv ({\neg} P)\lor ({\neg} Q).
</me>
Here we used DeMorgan's law. Therefore, the negation can be rewritten as:
<md>
<mrow>
   x \lt 3 \text{ or } x \gt 6.
</mrow>
</md>
</p>
</li>
<li>
<p>
 This sentence can be written as <m>R\implies (P\lor Q)</m> for
<md>
<mrow>
P: \amp \quad x \text{ is less than -2},
</mrow><mrow>
Q: \amp \quad x \text{ greater than 2},
</mrow><mrow>
R: \amp \quad x^2 \text{ is greater than 4}.
</mrow>
</md>.
Then its negation is:
<me>
{\neg} (R\Rightarrow ( Q\lor P))\equiv {\neg} \left({\neg} R\lor ( Q\lor P)\right)\equiv R\land (({\neg} Q)\land ({\neg} P)).
</me>
Here, first we used the equivalence of implication. Then DeMorgan's law and double negation. Thus, the negation can be rewritten as:
<md>
<mrow>
 \amp \text{The square of a real number } x \text{ is greater than 4 and }
</mrow><mrow>
 \amp  x  \text{ is greater than or equal to -2, and less than or equal to 2}.
</mrow>
</md>
</p>
</li>
<li>
<p>
  This sentence can be written as <m>P\implies (Q\implies R)</m> for
<md>
<mrow>
P:  \amp \quad f \text{ is differentiable everywhere},
</mrow><mrow>
Q:  \amp \quad x \text{ is a local maximum of } f,
</mrow><mrow>
R:  \amp \quad f'(x)=0.
</mrow>
</md>
Here, first we used the equivalence of implication. Then DeMorgan's law and double negation. Then its negation is:
<me>
{\neg} (P\Rightarrow ( Q\Rightarrow R))\equiv {\neg} \left({\neg} P\lor ({\neg} Q\lor R)\right)\equiv P\land (Q\land ({\neg} R)).
</me>
Here, first we used the equivalence of implication twice. Then DeMorgan's law and double negation. Hence, the negation can be rewritten as:
<md>
<mrow>
 \amp \text{A function } f \text{ is differentiable everywhere and } x\in\mathbb{R} \text{ is a local maximum of } f,
</mrow><mrow>
 \amp \text{ but } f'(x)\neq 0.
</mrow>
</md>
</p>

</li>
</ol>
</p>
</solution>
</exercise>
