<exercise>
<!-- source latex = 'intersection of graphs question.tex' -->
<!-- converted on 12/10/2021 at 13:44 -->
<statement>
<p>
Write down the set <m>F\cap G</m> where
<me>
F=\set{(x,x^2-3x+2)\in\mathbb{R}^2: x\in\mathbb R }
\qquad \text{and}\qquad
G=\set{ (a, a+2)\in\mathbb{R}^2: a\in\mathbb R }
</me>
by listing out all of its elements. Prove your answer.
</p>
</statement>
<answer>
<p>
The sets <m>F</m> and <m>G</m> may look like regular sets in <m>\mathbb R^2</m>, but we see that in both cases, the second item of each ordered pair is given as a function of the first coordinate. This suggests that <m>F</m> and <m>G</m>, indeed, can be seen as representing the graphs of the functions <m>f(x)=x^2-3x+2</m> and <m>g(x)=x+2</m> respectively. So, finding the intersection of these sets is the same as finding the intersection of these two graphs. Let's see how that works in the proof.
</p>

<p>
Any element in <m>F</m> is of the form <m>(x,x^2-3x+2)</m> and any element of <m>G</m> is of the form <m>(z,z+2)</m>. So if an element is in the intersection we must have that
<me>
(x,x^2-3x+2) = (z,z+2)
</me>
and so (since these are ordered pairs) <m>x=z</m> and <m>x^2-3x+2 = z+2</m>. Combining these we get the equation
<me>
x^2-3x+2=x+2
</me>
and so
<me>
  x^2-4x=0
</me>
which implies that <m>x=0,4</m>. So the points in the intersection are <m>\set{(0,2), (4,6)}</m>.
</p>
<p>
But, we still have to prove that
<me>
  F \cap G = \set{(0,2), (4,6)}
</me>
We do this in two ways, first we prove a sequence of set-equalities, and then second we show that each side is a subset of the other.
</p>

</answer>
<solution>


<proof><p>
We see that <m>F\cap G=\set{(a,b)\in\mathbb R^2\colon (a,b)\in F \text{ and } (a,b)\in G}</m>
<md>
<mrow>
F\cap G= \amp \set{(a,b)\in\mathbb R^2\colon (a,b)\in F \text{ and } (a,b)\in G}
</mrow><mrow>
= \amp \set{(a,b)\colon a,b\in\mathbb R, b=a^2-3a+2 \text{ and } b=a+2}
</mrow><mrow>
= \amp \set{(a,b)\colon a,b\in\mathbb R, b=a^2-3a+2=a+2}
</mrow><mrow>
= \amp \set{(a,b)\colon a,b\in\mathbb R, a^2-4a=0 \text{ and } b=a+2}
</mrow><mrow>
= \amp \set{(a,b)\colon a,b\in\mathbb R, (a=0 \text{ and } b=a+2=2), \text{ or } (a=4 \text{ and } b=a+2=6) }
</mrow><mrow>
= \amp \set{(0,2),(4,6)}
</mrow>
</md>
</p></proof>


<proof><p>
  We prove that
  <me>
    F \cap G \subseteq \set{(0,2), (4,6)}
    \qquad \text{and} \qquad
    \set{(0,2), (4,6)} \subseteq F\cap G
  </me>
  <ul>
<li>
<p>
 Let <m>(x,y) \in F\cap G</m>. So we know that <m>(x,y) \in F</m> and <m>(x,y) \in G</m>. Since <m>(x,y) \in F</m> we know that <m>x,y \in \mathbb{R}</m> so that <m>y=x^2-3x+2</m>. Then since <m>x,y \in G</m>, we know that <m>y=x+2</m>. Combining these two equations we see that we must have <m>x+2=x^2-3x+2</m> or, equivalently <m>x^2-4x=0</m>. This, in turn, implies that <m>x=0,4</m>. And thus <m>(x,y) = (0,2)</m> or <m>(x,y)=(4,6)</m>. In both cases <m>(x,y) \in \set{(0,2), (4,6)} </m> as required.
</p>
</li>
<li>
<p>
 Now let <m>(x,y) \in \set{(0,2), (4,6)}</m>. Then either <m>(x,y) = (0,2)</m> or <m>(x,y) = (4,6)</m>.
    <ul>
<li>
<p>
 Let <m>(x,y)=(0,2)</m>. Then since <m>2=0^2-3\cdot 0+2</m>, it follows that <m>(x,y) \in F</m>. Then, since <m>2=0+2</m>, we know that <m>(x,y) \in G</m>.
      </p></li>
<li>
<p>
 Very similarly, let <m>(x,y)=(4,6)</m>. Then since <m>6 = 4^2-3\cdot 4  + 2</m>, we know that <m>(x,y) \in F</m>. And since <m>6=4+2</m> we also know that <m>(x,y) \in G</m>.
    </p></li>
</ul>
    So in both cases, we have that <m>(x,y) \in F</m> and <m>(x,y) \in G</m>, and thus <m>(x,y) \in F \cap G</m> as required.
  </p></li>
</ul>
  Since both inclusions hold, the sets are equal.
</p></proof>

</solution>
</exercise>
