<exercise>
<!-- source latex = 'truth_table_question2.tex' -->
<!-- converted on 23/06/2021 at 20:59 -->
<statement>
<p>
Let <m>P</m> and <m>Q</m> be statements. Write out the truth tables for
<ol marker="(a)">
<li>
<p>
 <m> (\neg P)\implies Q </m>
</p></li>
<li>
<p>
 <m> (P\land Q)\lor \big((\neg P)\implies Q \big) </m>
</p></li>
<li>
<p>
 <m> P\land (\neg P)</m>
</p></li>
<li>
<p>
 <m> P\lor (\neg P)</m>
</p></li>
<li>
<p>
 <m> (P\implies Q) \iff (Q\implies P) </m>
</p>
</li>
</ol>
</p>
</statement>
<solution>
<p>
<ol marker="(a)">
<li>
<p>
 We can refer to the truth table for the implication, except this time the hypothesis is <m>\neg P</m> rather than <m>P</m>.
</p>
<tabular left="minor" right="minor" top="minor" bottom="minor" halign="center">
<row>
<cell>
<m>P</m>  </cell><cell>  <m>Q</m>  </cell><cell>  <m>\neg P</m>  </cell><cell>  <m>(\neg P)\implies Q</m></cell>
</row><row>
<cell>
T  </cell><cell>  T  </cell><cell>  F  </cell><cell>  T</cell>
</row><row>
<cell>
T  </cell><cell>  F  </cell><cell>  F  </cell><cell>  T</cell>
</row><row>
<cell>
F  </cell><cell>  T  </cell><cell>  T  </cell><cell>  T</cell>
</row><row>
<cell>
F  </cell><cell>  F  </cell><cell>  T  </cell><cell>  F</cell>
</row>
</tabular>
</li>
<li>
<p>
 We can use the truth table from part (a) to help figure out the new truth table.
</p>

<tabular left="minor" right="minor" top="minor" bottom="minor" halign="center">
<row>
<cell>
<m>P</m>  </cell><cell>  <m>Q</m>  </cell><cell>   <m>(\neg P)\implies Q</m>  </cell><cell>  <m>P\land Q</m>  </cell><cell>  <m>(P\land Q)\lor \big((\neg P)\implies Q \big)</m></cell>
</row><row>
<cell>
T  </cell><cell>  T   </cell><cell>  T  </cell><cell>  T  </cell><cell>  T</cell>
</row><row>
<cell>
T  </cell><cell>  F   </cell><cell>  T  </cell><cell>  F  </cell><cell>  T</cell>
</row><row>
<cell>
F  </cell><cell>  T   </cell><cell>  T  </cell><cell>  F  </cell><cell>  T</cell>
</row><row>
<cell>
F  </cell><cell>  F   </cell><cell>  F  </cell><cell>  F  </cell><cell>  F</cell>
</row>
</tabular>
</li>
<li>
<p>
 From the truth table, we see that <m>P\land (\neg P)</m> is always false.
</p>
<tabular left="minor" right="minor" top="minor" bottom="minor" halign="center"><row>
<cell>
<m>P</m>  </cell><cell>   <m>\neg P</m>  </cell><cell>  <m>P\land (\neg P) </m></cell>
</row><row>
<cell>
T  </cell><cell>  F  </cell><cell>  F</cell>
</row><row>
<cell>
F  </cell><cell>  T  </cell><cell>  F</cell>
</row>
</tabular>

</li>
<li>
<p>
 From the truth table, we see that <m>P\lor (\neg P)</m> is always true.
</p>

<tabular left="minor" right="minor" top="minor" bottom="minor" halign="center">
<row>
<cell>
<m>P</m>  </cell><cell>   <m>\neg P</m>  </cell><cell>  <m>P\lor (\neg P) </m></cell>
</row><row>
<cell>
T  </cell><cell>  F  </cell><cell>  T</cell>
</row><row>
<cell>
F  </cell><cell>  T  </cell><cell>  T</cell>
</row>
</tabular>

</li>
<li>
<p>
 From the truth table, we see that <m> (P\implies Q) \iff (Q\implies P) </m> is true only when <m>P</m> and <m>Q</m> have the same truth value.
</p>
<tabular left="minor" right="minor" top="minor" bottom="minor" halign="center">
<row>
<cell>
<m>P</m>  </cell><cell>  <m>Q</m>  </cell><cell>   <m>P\implies Q</m>  </cell><cell>  <m>Q\implies P</m>  </cell><cell>  <m> (P\implies Q) \iff (Q\implies P) </m></cell>
</row><row>
<cell>
T  </cell><cell>  T   </cell><cell>  T  </cell><cell>  T  </cell><cell>  T</cell>
</row><row>
<cell>
T  </cell><cell>  F   </cell><cell>  F  </cell><cell>  T  </cell><cell>  F</cell>
</row><row>
<cell>
F  </cell><cell>  T   </cell><cell>  T  </cell><cell>  F  </cell><cell>  F</cell>
</row><row>
<cell>
F  </cell><cell>  F   </cell><cell>  T  </cell><cell>  T  </cell><cell>  T</cell>
</row>
</tabular>

</li>
</ol>
</p>
</solution>
</exercise>
