<exercise>
<!-- source latex = 'truthtable.tex' -->
<!-- converted on 23/06/2021 at 20:53 -->
<statement>
<p>
Let <m>P</m> and <m>Q</m> be statements. Show that the truth table for <m>\neg(P\implies Q)</m> is the same as the truth table for <m>P\land\neg Q</m>.
</p>
</statement>
<solution>
<p>
We start with the truth table for <m>P\implies Q</m> given in <xref ref="def-implications"/>.
The next column (fourth column of the table) gives the truth table for <m>\neg(P\implies Q)</m>.
We compare this column to the last column of the table, which is the truth table for <m>P\land\neg Q</m>.
</p>

<tabular left="minor" right="minor" top="minor" bottom="minor" halign="center">
<row>
  <cell> <m>P</m>  </cell><cell>  <m>Q</m>  </cell><cell>  <m>P\implies Q</m>  </cell><cell>  <m>\neg(P\implies Q)</m>  </cell><cell>  <m>P\land\neg Q</m> </cell>
</row><row>
<cell>
T  </cell><cell>  T  </cell><cell>  T  </cell><cell>  F  </cell><cell>  F  </cell>
</row><row>
<cell> T  </cell><cell>  F  </cell><cell>  F  </cell><cell>  T  </cell><cell>  T  </cell>
</row><row>
<cell> F  </cell><cell>  T  </cell><cell>  T  </cell><cell>  F  </cell><cell>  F  </cell>
</row><row>
<cell> F  </cell><cell>  F  </cell><cell>  T  </cell><cell>  F  </cell><cell>  F  </cell>
</row>
</tabular>

<!-- <p>
Let's go over some examples from the last column of the table: when both <m>P</m> and <m>Q</m> are true, <m>P\land\neg Q</m> is false, because <m>\neg Q</m> is false.
When <m>P</m> is true and <m>Q</m> is false, both <m>P</m> and <m>\neg Q</m> are true, and therefore <m>P\land \neg Q</m> is true.
</p> -->

</solution>
</exercise>
