<exercise>
<!-- source latex = '8 divides 3^{2n}-1.tex' -->
<!-- converted on 08/11/2021 at 10:43 -->
<statement>
<p>
Let <m>m\in\mathbb{N}</m>, with <m>m</m> even. Show that <m>8</m> divides <m>3^m-1</m>.
</p>
</statement>
<hint>
<p>
The even-ness of the exponent is required, otherwise the statement is simply not true:
<me>
  3^3 -1 = 27-1 = 26
</me>
and 8 definitely does not divide 26. Rephrase things to take advantage of what you know about even numbers.
</p>
</hint>
<answer>
<p>
We want to prove this statement by induction. As written, we want to prove something about all <m>m\in\mathbb{N}</m>, with <m>m</m> even.
In order to prove this by induction, however, we need reformulate the statement into something that we want to prove for all natural numbers instead.
We can do this by writing <m>m=2n</m> for <m>n\in\mathbb{N}</m>. Then we need to prove that <m>8</m> divides <m>3^{2n}-1</m>. We can prove this by induction on <m>n</m>.
</p>
<p>
<ul>
<li>
<p>
 Base case: Take <m>n=1</m>. Then <m> 3^{2\cdot n}-1 =9-1=8, </m>, so the result holds.
</p></li>
<li>
<p>
 Inductive step: Assume that
<me> 8\mid 3^{2k}-1. </me>
We want to show that
<me> 8\mid 3^{2(k+1)}-1. </me>
Our assumption implies that there is some <m>\ell</m> so that
<me>
  3^{2k}-1 = 8 \ell
</me>
Rephrasing this we have <m>3^{2k} = 8\ell+1</m>. Notice that this implies that
<me>
  3^{2k+2} = 72\ell + 9
</me>
and thus
<me>
  3^{2k+2}-1 = 72\ell + 8 = 8(9\ell + 1)
</me>
giving us the divisibilty result we need.
</p>
</li>
<li>
<p>
 Inductive step <mdash/> another way: Another way to approach the inductive step is to consider the difference between
<me>
  (3^{2k}-1) \qquad \text{and} \qquad (3^{2k+2}-1).
</me>
If that difference is a multiple of 8 then we can infer the result we need. So again, we assume that <m>8 \mid 3^{2k}-1</m>, and then consider the difference:
<me>
(3^{2k+2}-1) - (3^{2k}-1)
= 3^{2k+2} - 3^{2k} = 9 \cdot 3^{2k} - 3^{2k} = 8\cdot 3^{2k}.
</me>
Then since <m>8 \mid 3^{2k}-1</m> we can write it as <m>8\ell</m> for some integer <m>\ell</m>, and so
<me>
(3^{2k+2}-1) - \underbrace{(3^{2k}-1)}_{=8\ell} = 8 \cdot 3^{2k}
</me>
and so, with a little rearranging:
<me>
(3^{2k+2}-1) = 8 \ell + 8 \cdot 3^{2k}.
</me>
So we see that <m>3^{2(k+1)}-1</m> is divisible by <m>8</m>.
</p></li>
</ul>
</p>
<p>
Now we can write the formal proof up:
</p>
</answer>

<solution>
  <proof>
<p>
Let <m>n\in\mathbb{N}</m>.
We proceed by induction on <m>n</m>. When <m>n=1</m>, we have
<me> 3^{2\cdot 1}-1 =9-1=8, </me>
which is divisible by <m>8</m>. Now suppose that the result holds for <m>n=k</m>, so
<me> 8 \mid 3^{2k}-1. </me>
So we can write <m>3^{2k}-1 = 8\ell</m> for some <m>\ell \in \mathbb{Z}</m>. Now, notice that
<md>
<mrow>
  3^{2k+2} -1  \amp = 9 \cdot 3^{2k} -1  
</mrow><mrow>
   \amp = 8\cdot 3^{2k} + (3^{2k} -1)  
</mrow><mrow>
   \amp = 8\cdot 3^{2k} + 8\ell
</mrow>
</md>
Thus <m>8</m> divides <m>3^{2(k+1)}</m> as required.
</p>
<p>
Therefore, by induction, <m>8</m> divides <m>3^{2n}-1</m> for all <m>n\in\mathbb{N}</m>. Hence, equivalently, <m>8</m> divides <m>3^m-1</m> for any even <m>m\in\mathbb{N}</m>.
</p></proof>

</solution>
</exercise>
