<exercise xml:id="ex_binom_thm">
<!-- source latex = 'binomial_thm.tex' -->
<!-- converted on 12/10/2021 at 14:06 -->
<statement>
<p>
Let <m>n,r \in \mathbb{Z}</m> so that <m>0 \leq r \leq n</m>. We define the binomial coefficient
<me>
  \binom{n}{r}  = \frac{n!}{(n-r)! r!}.
</me>
</p>
<p>
<ol marker="(a)">
<li>
<p>
 Prove that the binomial coefficients satisfy Pascal's identity:
  <me>
    \binom{n+1}{r} = \binom{n}{r} + \binom{n}{r-1}
    \qquad \text{for } 0 \lt r \leq n
  </me>
  </p></li>
<li>
<p>
 and so prove, using induction, the Binomal Theorem:
  <me>
    (a+b)^n = \sum_{k=0}^n \binom{n}{k} a^{n-k} b^k
  </me>
  for any <m>a,b \in \mathbb{R}</m> and any <m>n \in \mathbb{N}</m>.
</p>
</li>
</ol>
</p>
</statement>
<hint>
<p>
<ul>
<li>
<p>
 For Pascal's identity, rewrite the binomials as factorials and juggle carefully.
  </p></li>
<li>
<p>
 For the binomial theorem, expand and group carefully. The following might also be handy
  <md>
<mrow>
    \binom{n}{0} = \binom{n}{n} = 1.
  </mrow>
</md>
  Also, be careful around the edges of your expanded sums.
</p></li>
</ul>
</p>
</hint>
<solution>
<p>
We prove each result in turn. First, Pascal's identity:
</p>

<proof><p>
  Let <m>n,r</m> be as given, then
  <md>
<mrow>
    \binom{n}{r} + \binom{n}{r-1}
     \amp = \frac{n!}{(n-r)! r!} + \frac{n!}{(n-r+1)! (r-1)!}
</mrow><mrow>
     \amp = \frac{n! (n-r+1)}{(n-r+1)! r!} + \frac{n! \cdot r}{(n-r+1)! r!}
</mrow><mrow>
     \amp = \frac{n!}{(n-r+1)! r!} \left(n-r+1 + r \right)
</mrow><mrow>
     \amp = \frac{n! (n+1)}{(n+1-r)! r!}
</mrow><mrow>
     \amp = \frac{(n+1)!}{( (n+1)-r)! r!}
</mrow><mrow>
     \amp = \binom{n+1}{r}
  </mrow>
</md>
  as required.
</p></proof>

<p>
Next, the Binomial Theorem:
</p>

<proof><p>
  Let <m>a,b</m> be as stated, and then we prove the result by induction on <m>n</m>.
<ul>
<li>
<p>
 When <m>n=1</m> we have that <me>
  (a+b)^1 = a+b = \binom{1}{0} a + \binom{1}{1} b
  </me>
  and so the base case holds.
  </p></li>
<li>
<p>
 Now assume that the result holds for some <m>n = \ell \in \mathbb{N}</m> and we show that it holds for <m>n = \ell+1</m>. Start with
  <me>
    (a+b)^\ell = \sum_{k=0}^\ell \binom{\ell}{k} a^{\ell-k} b^k.
  </me>
  Multiplying both sides by <m>(a+b)</m> gives:
  <md>
<mrow>
    (a+b)^{\ell+1}  \amp = (a+b)\sum_{k=0}^\ell \binom{\ell}{k} a^{\ell-k} b^k
</mrow><mrow>
     \amp = \sum_{k=0}^\ell \binom{\ell}{k} a^{\ell-k} b^k (a+b)
</mrow><mrow>
     \amp = \sum_{k=0}^\ell \binom{\ell}{k} a^{\ell-k+1} b^k + \sum_{k=0}^\ell \binom{\ell}{k} a^{\ell-k} b^{k+1}
     </mrow><intertext>Extract out the very first and very last terms</intertext><mrow>
     \amp =
    \binom{\ell}{0} a^{\ell+1}
    + \sum_{k=1}^\ell \binom{\ell}{k} a^{\ell-k+1} b^k
    + \sum_{k=0}^{\ell-1} \binom{\ell}{k} a^{\ell-k} b^{k+1}
    + \binom{\ell}{\ell} a^0 b^{\ell+1}
    </mrow><intertext>re-index the second sum to make it start from 0 by replacing <m>k</m> with <m>k-1</m></intertext><mrow>
     \amp =
    a^{\ell+1}
    + \sum_{k=1}^{\ell} \binom{\ell}{k} a^{\ell-k+1} b^{k}
    + \sum_{k=1}^{\ell} \binom{\ell}{k-1} a^{\ell-k+1} b^{k}
    + a^0 b^{\ell+1}
    </mrow><intertext>If we group-together terms with similar powers of <m>a,b</m>, we get</intertext><mrow>
     \amp =
    a^{\ell+1}
    + \sum_{k=1}^{\ell} \left[ \binom{\ell}{k} + \binom{\ell}{k-1} \right] a^{\ell-k+1} b^{k+1}
    + b^{\ell+1}
    </mrow><intertext>then, Pascal's identity gives</intertext><mrow>
     \amp =
    a^{\ell+1}
    + \sum_{k=1}^{\ell} \binom{\ell+1}{k} a^{\ell+1-k} b^{k}
    + b^{\ell+1}
    </mrow><intertext>Finally, since <m>\binom{\ell+1}{0}=\binom{\ell+1}{\ell+1}=1 </m>, we have</intertext><mrow>
     \amp =
    \binom{\ell+1}{0} a^{\ell+1} b^0
    + \sum_{k=1}^{\ell} \binom{\ell+1}{k} a^{\ell+1-k} b^{k}
    + \binom{\ell+1}{\ell+1} a^0 b^{\ell+1}
</mrow><mrow>
     \amp = \sum_{k=0}^{\ell+1} \binom{\ell+1}{k} a^{\ell+1-k} b^{k}
  </mrow>
</md>
  as required.
</p>
<p>
  Since the base-case and inductive step hold, the result follows by induction.
</p></li>
</ul>
</p>
</proof>

</solution>
</exercise>
