<exercise xml:id="ex_distributive_law">
<!-- source latex = 'distributive_law.tex' -->
<!-- converted on 08/11/2021 at 10:42 -->
<statement>
<p>
The <em>distributive law</em> says that for any real numbers <m>a,b,c</m>, we have
<me> a\cdot(b+c)=a\cdot b+a\cdot c. </me>
Use induction to show that for any <m>n\geq 2</m> and any real numbers <m>a,b_1,b_2\dots,b_n</m>
<me> a\cdot(b_1+b_2+\dots+b_n)=a\cdot b_1+a\cdot b_2+\dots+a\cdot b_n. </me>
</p>
</statement>

<!-- <hint></hint> -->


<answer>
 <p>
We want to prove this statement by induction on <m>n</m>.
<ul>
<li>
<p>
 Base case: Take <m>n=2</m>. Then the distributive law gives the result in this case.
</p></li>
<li>
<p>
 Inductive step: Assume that the result holds for <m>n=k</m>, and let <m>a,b_1,\dots,b_k,b_{k+1}</m> be real numbers.
The inductive step tells us that
<me> a\cdot(b_1+b_2+\dots+b_k)=a\cdot b_1+a\cdot b_2+\dots+a\cdot b_k, </me>
which we want to use to show that
<me> a\cdot(b_1+b_2+\dots+b_k+b_{k+1})=a\cdot b_1+a\cdot b_2+\dots+a\cdot b_k+a\cdot b_{k+1}. </me>
We want to consider the sum <m>b_1+b_2+\dots+b_k+b_{k+1}</m> as the sum of two elements, <m>b_1+b_2+\dots+b_k</m> and <m>b_{k+1}</m>.
Then the distributive law tells us that
<me> a\cdot((b_1+b_2+\dots+b_k)+b_{k+1})=a\cdot(b_1+b_2+\dots+b_k)+a\cdot b_{k+1}. </me>
Then we can apply the inductive hypothesis to obtain the desired result.
</p></li>
</ul>
</p>
<p>
Now we can write the formal proof up:
</p>
</answer>
<solution>
  <proof>
<p>
Let <m>n\in\mathbb{N}</m>.
We proceed by induction on <m>n</m>. When <m>n=2</m>, the result holds by the distributive law. Now assume the result holds for <m>n=k</m>, and suppose that
<m>a,b_1,b_2,\dots,b_k,b_{k+1}</m> are real numbers. Then
<me> a\cdot(b_1+b_2+\dots+b_k+b_{k+1})=a\cdot((b_1+b_2+\dots+b_k)+b_{k+1})=a\cdot(b_1+b_2+\dots+b_k)+a\cdot b_{k+1} </me>
by the distributive law. But by inductive hypothesis,
<me>a\cdot(b_1+b_2+\dots+b_k)+a\cdot b_{k+1}=a\cdot b_1+a\cdot b_2+\dots+a\cdot b_k+a\cdot b_{k+1}. </me>
and so
<me> a\cdot(b_1+b_2+\dots+b_k+b_{k+1})=a\cdot b_1+a\cdot b_2+\dots+a\cdot b_k+a\cdot b_{k+1}. </me>
Therefore, the result holds for any <m>n\in\mathbb{N}</m>, <m>n\geq 2</m>.
</p></proof>

<p>
This proof gives us a general strategy on how we may use induction to extend a result between two objects to a result between any finite number of objects.
</p>
</solution>
</exercise>
