<exercise>
<!-- source latex = 'factorial_as_integral.tex' -->
<!-- converted on 08/11/2021 at 10:45 -->
<statement>
<p>
Let <m>n\in\mathbb{Z}</m>, <m>n\geq0</m>.
<ol marker="(a)">
<li>
<p>
 Use induction and l'Hôpital's rule to show that
<me> \lim_{x\to\infty}x^ne^{-x}=0. </me>
</p></li>
<li>
<p>
 Show that
<me> n! = \int_0^\infty x^ne^{-x}\mathrm{d}x. </me>
</p>
</li>
</ol>
For this question
<ul>
<li>
<p>
 recall that <m>0!=1</m>, and
  </p></li>
<li>
<p>
 you may use basic facts about limits and integration from your Calculus-1 course.
</p></li>
</ul>
</p>
</statement>
<hint>
<p>
For (b) try integration by parts.
</p>
</hint>

<answer>

<p>
<ol marker="(a)">
<li>
<p>
 We'll prove this by induction on <m>n</m>.
</p>
<p>
<ul>
<li>
<p>
 Base case: take <m>n=0</m>. Then
<me> \lim_{x\to\infty}x^ne^{-x}=\lim_{x\to\infty}e^{-x}=0. </me>
</p></li>
<li>
<p>
 Inductive step: Assuming
<me> \lim_{x\to\infty}x^ke^{-x}=0, </me>
we want to show that
<me> \lim_{x\to\infty}x^{k+1}e^{-x}=0. </me>
Rewrite the limit as
<me> \lim_{x\to\infty}\frac{x^{k+1}}{e^{x}} </me>
Then both the numerator and the denominator go to infinity as <m>x\to\infty</m>. Then we can use l'Hôpital's rule to obtain
<me> \lim_{x\to\infty}\frac{x^{k+1}}{e^{x}}=\lim_{x\to\infty}\frac{(k+1)x^{k}}{e^{x}}. </me>
Now we have a limit that almost looks like the one from the inductive hypothesis; we just need to pull out the constant factor of <m>k+1</m>, and then
apply the inductive hypothesis:
<me> \lim_{x\to\infty}\frac{x^{k+1}}{e^{x}}=(k+1)\lim_{x\to\infty}\frac{x^{k}}{e^{x}}=(k+1)\cdot0=0. </me>
</p></li>
</ul>
</p>
</li>
<li>
<p>
 We'll prove this by induction on <m>n</m>.
</p>
<p>
<ul>
<li>
<p>
 Base case: take <m>n=0</m>. Then
<me> \int_0^\infty x^ne^{-x}\mathrm{d}x =\int_0^\infty e^{-x}\mathrm{d}x  </me>
Evaluating this integral yields
<me> \int_0^\infty e^{-x}\mathrm{d}x = \lim_{t\to\infty}(-e^{-x})\Big]_0^t = 1. </me>
And since <m>1=0!</m> the base case holds.
</p></li>
<li>
<p>
 Inductive step: Suppose that
<me> k! = \int_0^\infty x^ke^{-x}\mathrm{d}x.</me>
We want to use this equation in order to show that
<me> (k+1)! = \int_0^\infty x^{k+1}e^{-x}\mathrm{d}x.</me>
We can connect the integral in the equation for <m>(k+1)!</m> to the integral in the equation for <m>k!</m> by using integration by parts, because <m>\frac{d}{\mathrm{d}x}x^{k+1}=(k+1)x^k</m>.
Indeed, by integration by parts,
<md>
<mrow>
\int_0^\infty x^{k+1}e^{-x}\mathrm{d}x \amp =(-x^{k+1}e^{-x})\Big]_0^\infty +(k+1)\int_0^\infty x^ke^{-x}\mathrm{d}x
</mrow><mrow>
 \amp =\lim_{t\to\infty} \left(-t^{k+1}e^{-t}\right)+0^{k+1}e^{-0} +(k+1)\int_0^\infty x^ke^{-x}\mathrm{d}x
</mrow>
<intertext>We then use our result from (a) to evaluate that limit, giving</intertext><mrow>
 \amp = 0 +(k+1)\int_0^\infty x^ke^{-x}\mathrm{d}x
</mrow>
</md>
Now we're left with <m>(k+1)</m> times the integral that we've assumed is equal to <m>k!</m> in the inductive hypothesis. But this gives exactly the equation that we wanted to show!
</p></li>
</ul>
</p>
</li>
</ol>
</p>

</answer>

<solution>

<proof><title>Proof of (a)</title>
<p>
Let <m>n\in\mathbb{Z}</m>, <m>n\geq0</m>. We proceed by induction on <m>n</m>. First assume <m>n=0</m>. Then
<me> \lim_{x\to\infty}x^ne^{-x}=\lim_{x\to\infty}e^{-x}=0, </me>
and so the result holds. Next suppose the result holds for <m>n=k</m>, so that
<me> \lim_{x\to\infty}x^ke^{-x}=0. </me>
By l'Hôpital's rule,
<me> \lim_{x\to\infty}x^{k+1}e^{-x}=\lim_{x\to\infty}\frac{x^{k+1}}{e^{x}}=\lim_{x\to\infty}\frac{(k+1)x^{k}}{e^{x}}. </me>
Pulling out the constant, and applying the inductive hypothesis, we have
<me> \lim_{x\to\infty}\frac{x^{k+1}}{e^{x}}=(k+1)\lim_{x\to\infty}\frac{x^{k}}{e^{x}}=(k+1)\cdot0=0. </me>
Therefore the result holds for <m>n=k+1</m>, and by induction, for any <m>n</m>.
</p></proof>




<proof><title>Proof of (b)</title>
<p>
Let <m>n\in\mathbb{Z}</m>, <m>n\geq0</m>. We proceed by induction on <m>n</m>. First assume <m>n=0</m>. Then
<me> \int_0^\infty x^ne^{-x}\mathrm{d}x =\int_0^\infty e^{-x}\mathrm{d}x = \lim_{t\to\infty}(-e^{-x})\Big]_0^t = 1=0!. </me>
Next suppose that the result holds for <m>n=k</m>; that is,
<me> k! = \int_0^\infty x^ke^{-x}\mathrm{d}x.</me>
Then, by integration by parts,
<md>
<mrow>
\int_0^\infty x^{k+1}e^{-x}\mathrm{d}x \amp =(-x^{k+1}e^{-x})\Big]_0^\infty +(k+1)\int_0^\infty x^ke^{-x}\mathrm{d}x
</mrow><mrow>
 \amp =\lim_{t\to\infty} \left(-t^{k+1}e^{-t}\right)+0^{k+1}e^{-0} +(k+1)\int_0^\infty x^ke^{-x}\mathrm{d}x
</mrow><mrow>
 \amp = 0 +(k+1)\int_0^\infty x^ke^{-x}\mathrm{d}x
</mrow>
</md>
where we have used the fact that
<me>
\lim_{x \to \infty} x^k e^{-x} = 0.
</me>
which we proved in (a). Now using the induction hypothesis, we therefore have
<me> \int_0^\infty x^{k+1}e^{-x}\mathrm{d}x=(k+1)\int_0^\infty x^ke^{-x}\mathrm{d}x=(k+1)k!=(k+1)!. </me>
Thus, by induction, the result holds for all <m>n</m>.
</p></proof>

</solution>
</exercise>
