<exercise>
<statement>
  <p>
    Let <m>F_k</m> be the <m>k^\mathrm{th}</m> Fibonacci number, and
    let <m>q \in \mathbb{N}</m>. Show that <m>F_q \mid F_{qn}</m> for
    all <m>n \in \mathbb{N}</m>. This generalises <xref ref="prop-fib3"/>.
</p>
</statement>
<hint>
  <p>
    The proof of <xref ref="prop-fib3"/> works because <m>5</m> is a Fibonacci number. See how you might generalise what is happening in the proof.
  </p>
</hint>
<answer>
  <p>
    Let's try making this work with <m>F_7 = 13</m>. That is, we want
    to show that <m>F_7 \mid F_7n</m>.  Se we'll assume that <m>F_7
    \mid F_{7k}</m> and then we'll try to show that this implies that
    <m>F_7 \mid F_{7k+7}</m>. Now, from the definition of the
    Fibonacci numbers, we can write <m>F_{7k+7}</m> in terms of
    <m>F_{7k+6}</m> and <m>F_{7k+5}</m>:
    <me>
      F_{7k+7} = F_{7k+6}+F_{7k+5}
    </me>
    and then similarly expand <m>F_{7k+6} = F_{7k+5}+F_{7k+4}</m>, so:
    <me>
      F_{7k+7} = 2F_{7k+5}+F_{7k+4}
    </me>
    and keep going:
    <md>
      <mrow>F_{7k+7} \amp = 2F_{7k+5}+F_{7k+4} \amp \text{expand } F_{7k+5}</mrow>
      <mrow> \amp= 3F_{7k+4} + 2 F_{7k+3} \amp \text{expand } F_{7k+4}</mrow>
      <mrow> \amp= 5F_{7k+3} + 3 F_{7k+2} \amp \text{expand } F_{7k+3}</mrow>
      <mrow> \amp= 8F_{7k+2} + 5 F_{7k+1} \amp \text{expand } F_{7k+2}</mrow>
      <mrow> \amp= 13F_{7k+1} + 8 F_{7k}</mrow>
    </md>
    Now since, by assumption <m>13=F_{7} \mid F_{7k}</m>, we are done.
  </p>
  <p>
    Notice that each time we expand and regroup the terms we get another Fibonacci number. So, let us try to write this more explicitly in terms of Fibonacci numbers:
    <md>
      <mrow>F_n \amp = 1 \cdot F_{n-1} + 1 \cdot F_{n-2}</mrow>
      <mrow> \amp = F_2 \cdot F_{n-1} + F_1 \cdot F_{n-2}</mrow>
      <mrow> \amp = F_3 \cdot F_{n-2} + F_2 \cdot F_{n-3} </mrow>
      <mrow> \amp = F_4 \cdot F_{n-3} + F_3 \cdot F_{n-4} </mrow>
      <mrow> \amp = F_5 \cdot F_{n-4} + F_4 \cdot F_{n-5} </mrow>
    </md>
    So we might try to show, more generally, that
    <me>
      F_n = F_{\ell} \cdot F_{n-\ell+1} + F_{\ell-1} \cdot F_{n-\ell}
    </me>
    or equivalently (after substituting <m>n \mapsto n+\ell</m>)
    <me>
      F_{n+\ell} = F_{\ell} \cdot F_{n+1} + F_{\ell-1} \cdot F_{n}.
    </me>
    Setting <m>n=7k, \ell=7</m> in this gives us 
    <me>
      F_{7k+7} = F_{7} \cdot F_{7k+1} + F_{6} \cdot F_{7k}
    </me>
    which is precisely what we need.
  </p>
</answer>
<solution>
  <proof>
    <p>
      Let <m>n \in \mathbb{N}</m>. We prove, using strong induction, that for all <m>\ell \in \mathbb{N}</m>
      <me>
      F_{n+\ell} = F_{\ell} \cdot F_{n+1} + F_{\ell-1} \cdot F_{n}.
      </me>
      and then use this to prove the result.
      <ul>
	<li>
	  <p>
	    Base case: When <m>\ell=1</m> we have
	    <me>
	      F_{n+1} = F_1 \cdot F_{n+1} + F_0 \cdot F_{n}
	    </me>
	    and since <m>F_0=0, =F_1=1</m>, this follows.
	  </p>
	</li>
	<li>Inductive step: 
	  Now assume that 
	  <me>
	    F_{n+k} = F_{k} \cdot F_{n+1} + F_{k-1} \cdot F_{n}.
	  </me>
	  holds for all <m>k \leq \ell</m>. Then
	  <md>
	    <mrow>F_{n+\ell+1} \amp = F_{n+\ell} + F_{n+\ell-1}</mrow>
	    <mrow>\amp =
	    (F_{\ell} \cdot F_{n+1} + F_{\ell-1} \cdot F_{n}) + (F_{\ell-1} \cdot F_{n} + F_{\ell-2} \cdot F_{n-1})
	    </mrow>
	    <mrow>
	      \amp = (F_{\ell}+F_{\ell-1} ) \cdot F_{n} + (F_{\ell-1}+F_{\ell-2}) \cdot F_{n-1}
	    </mrow>
	    <mrow>
	      \amp = F_{\ell+1} \cdot F_{n} + F_{\ell} \cdot F_{n-1}
	    </mrow>
	  </md>
	  as required.
	</li>
      </ul>
      Thus
      <me>
      F_{n+\ell} = F_{\ell} \cdot F_{n+1} + F_{\ell-1} \cdot F_{n}.	
      </me>
      holds for all <m>\ell \in\mathbb{N}</m>.      
    </p>
    <p>
      Now we prove the main result by induction.
      <ul>
	<li>Base case: Since <m>F_q \mid F_q</m> the case case is true.</li>
	<li>
	  <p>
	    Inductive step: Assume that
	    <me>
	      F_q \mid F_{qn}
	    </me>
	    and consider <m>F_{qn+q}</m>. By the inductive result we proved above (with <m>n \mapsto qn</m> and <m>\ell \mapsto q</m>) we know that
	    <me>
	      F_{qn+q} = F_{q+1} \cdot F_{qn} + F_q \cdot F_{qn-1}
	    </me>
	    Now since <m>F_q \mid F_{qn}</m> by assumption, this shows that <m>F_q \mid F_{qn+q}</m> as required.
	  </p>
	</li>
      </ul>
      Thus <m>F_q \mid F_{qn}</m> for all <m>n \in \mathbb{N}</m>.
    </p>
  </proof>

  <!-- <proof> -->
  <!--   <p> -->
  <!--     Fix <m>q \in \mathbb{N}</m>. We prove the result by -->
  <!--     induction. When <m>n=1</m> the result holds since <m>F_q \mid -->
  <!--     F_q</m>. -->
  <!--   </p> -->
  <!--   <p> -->
  <!--     Now assume that <m>F_q \mid F_{qk}</m>. Now -->
  <!--     <md> -->
  <!--       <mrow>F_{qk+q} \amp= F_{qk+q-1} + F_{qk+q-2} </mrow> -->
  <!--       <mrow> \amp= (F_{qk+q-2} + F_{qk+q-3}) + F_{qk+q-2} = 2F_{qk+q-2}+F_{qk+q-3}</mrow> -->
  <!--       <mrow> \amp= 2(F_{qk+q-3}+F_{qk+q-4}) + F_{qk+q-3} = 3 F_{qk+q-3} + 2F_{qk+q-4}</mrow> -->
  <!--       <mrow> \amp= 3(F_{qk+q-4}+F_{qk+q-5}) + 2F_{qk+q-3} = 5 F_{qk+q-4} + 3F_{qk+q-5}</mrow> -->
  <!--       <mrow> \amp= 5(F_{qk+q-5}+F_{qk+q-6}) + 3F_{qk+q-3} = 8 F_{qk+q-5} + 5F_{qk+q-6}</mrow> -->
  <!--       <mrow> \amp=\vdots  </mrow> -->
  <!--       <mrow> \amp = F_{j} F_{qk+q-j-1} + F_{j-1} F_{qk+q-j} </mrow> -->
  <!--       <mrow> \amp=\vdots  </mrow> -->
  <!--       <mrow> \amp=  F_q F_{qk+1} + F_{q-1} F_{qk}</mrow> -->
  <!--     </md> -->
  <!--     Then since <m>F_q \mid F_{qk}</m> it follows that <m>F_q \mid F_{qk+q}</m> as required. -->
  <!--     The result follows by induction. -->
  <!--   </p> -->
  <!-- </proof> -->
</solution>
</exercise>
