<exercise>
<!-- source latex = 'induction_adr1.tex' -->
<!-- converted on 12/08/2021 at 20:08 -->
<statement>
<p>
Let <m>n \in \mathbb{N}</m> so that <m>n \geq 2</m>. Use mathematical induction to prove that
<me>
  n!  \leq n^n
</me>
Recall that <m>n! = n \cdot(n-1) \cdot(n-2)\cdots 2 \cdot 1</m>.
</p>
</statement>
<hint>
<p>
Write out the statement for <m>n=k</m> and <m>n=k+1</m> and try to work out how to make the left-hand side of the first statement look like the left-hand side of the second statement.
</p>
</hint>
<answer>
<p>
When <m>n=k</m> the statement is
<me>
k! \leq k^k
</me>
and we will need to prove that when <m>n=k+1</m>
<me>
(k+1)! \leq (k+1)^(k+1)
</me>
Notice that <m>(k+1)! = k! \cdot (k+1)</m>, and so we can make the first statement look like the second by multiplying by <m>(k+1)</m>.
</p>
</answer>

<solution>
<proof><p>
We prove the result by induction.
<ul>
<li>
<p>
 Base case: when <m>n=2</m> we have <m>n! = 2 \cdot 1 = 2</m> and <m>n^n = 2^2 = 4</m>. Since <m>2 \leq 4</m>, the result holds when <m>n=2</m>.
  </p></li>
<li>
<p>
 Inductive step: Assume the result holds when <m>n=k\geq 2</m>. Then we have
  <md>
<mrow>
      k!  \amp  \leq k^k  \amp  \text{multiply both sides by } k+1 \gt 0
</mrow><mrow>
      (k+1)!  \amp  \leq (k+1) \cdot k^k  \amp  \text{since } k \lt k+1
</mrow><mrow>
       \amp  \leq (k+1) \cdot (k+1)^k
</mrow><mrow>
       \amp  = (k+1)^{k+1}
  </mrow>
</md>
  That is <m>(k+1)! \leq (k+1)^{k+1}</m>, so the result holds when <m>n=k+1</m>.
</p></li>
</ul>
Since the base case and inductive step both hold, the result follows by induction.
</p></proof>

</solution>
</exercise>
