<exercise>
<!-- source latex = 'merge_sort.tex' -->
<!-- converted on 19/11/2021 at 10:51 -->
<statement>
<p>
For <m>n \in \mathbb{N}</m>, consider the recurrence
<me>
  T(1)=1 \qquad\text{and for } n \geq 2 \qquad T(n) = 2 T\left( \left\lfloor \frac{n}{2}  \right\rfloor \right) + n
</me>
The first few values of <m>T(n)</m> are
<me>
  1, 4, 5, 12, 13, 16, 17, 32, 33, \dots
</me>
Use strong induction to prove that for <m>n \geq 1 </m>, <m> T(n) </m> satisfies the bound
<me>
    T(n) \leq  n \log_2 n + n.
</me>
</p>
<p>
Note that the logarithm has base 2, and that the floor function, <m> \lfloor x\rfloor</m>, gives the largest integer smaller or equal to <m>x</m>.
</p>
<p>
Recurrences such as this one appear very frequently in the analysis of <q>divide and conquer</q> algorithms. That class of algorithms (roughly speaking) work by repeatedly splitting a larger problem into smaller pieces until they can be solved trivially. The interested reader should search-engine their way to more information.
</p>
</statement>
<hint>
<p>
You can simplify the analysis of the floor function by studying even and odd values separately.
</p>
</hint>
<solution>

<proof><p>
  We prove the result by strong induction.
  <ul>
<li>
<p>
 When <m>n=1</m> we have <m>T(1)=1</m> and since <m>1 \log_2 1 +1 = 1</m>, the result holds.
    </p></li>
<li>
<p>
 Now assume that the result holds for all <m>1 \leq k \leq \ell</m> and we wish to show that it holds for <m>k= \ell+1</m>. Since the recurrence is slightly different for even or odd <m>k=\ell+1</m>, we split into two cases.
    <ul>
<li>
<p>
 Assume that <m>k=\ell+1 = 2j</m>, then
      <md>
<mrow>
        T(k)  \amp = 2T(j) + k 
</mrow><mrow>
         \amp  \leq 2\left( j \log_2(j) + j \right) + k 
</mrow><mrow>
         \amp  = 2j \log_2(j) + 2j + k 
</mrow><mrow>
         \amp = k \log_2\left(\frac{2j}{2}\right) + 2k 
</mrow><mrow>
         \amp = k \left( \log_2(k) - \log_2(2) \right) +2k 
</mrow><mrow>
         \amp = k\log_2(k) + k,
       </mrow>
</md>
       since <m> \log_2(2) = 1</m>.
       </p></li>
<li>
<p>
 Now assume that <m>k=\ell+1 = 2j+1</m>, then
       <md>
<mrow>
         T(k)  \amp = 2T(j) + k 
</mrow><mrow>
          \amp  \leq 2\left( j \log_2(j) + j \right) + k 
</mrow><mrow>
          \amp  = 2j \log_2(j) + 2j + k 
</mrow><mrow>
          \amp = k \log_2\left(\frac{2j}{2}\right) + 2k-1 
</mrow><mrow>
          \amp = k\log_2(k) + k-1 \lt k\log_2(k)+k
        </mrow>
</md>
        where again we have used <m> \log_2(2) = 1</m>.
    </p></li>
</ul>
    In both cases the inductive step holds.
  </p></li>
</ul>
  Since both the base case and inductive step are true, the result follows by induction.
</p>
</proof>

</solution>
</exercise>