<exercise>
<!-- source latex = 'Sum of cubes is the square of the sum question.tex' -->
<!-- converted on 12/08/2021 at 20:10 -->
<statement>
<p>
Prove that, <m>\forall n\in\mathbb{N}</m>, <m>\displaystyle \sum_{k=1}^n k^3=\left( \sum_{k=1}^n k \right)^2</m>.
</p>
</statement>
<hint>
<p>
The sum <m> \sum\limits_{k=1}^n k</m> is a very standard result and is in the main text. You can use that result without proof.
</p>
</hint>
<answer>
<p>
Here we see that we have a statement we want to show is true for all <m>n\in\mathbb N</m>. In the previous chapters we have seen that to show such statements we assume that <m>n\in\mathbb N</m> and try to show the conclusion. Moreover, since the hypothesis is broad, we would probably need to look at cases. But, in this question, it is not clear what the cases should be. Instead, we can also apply mathematical induction. We see that this equation doesn't seem to give us a formula, but instead gives us two expressions. However, we know what the right hand side is equal to.
</p>
<p>
We know that <m>\displaystyle{\sum\limits_{k=1}^m k}=\dfrac{m(m+1)}{2}</m> (see <xref ref="prop-sum-of-int"/>). This means that what we wat to show now becomes
<me>
\sum\limits_{k=1}^{n} k^3=\frac{n^2(n+1)^2}{4}.
</me>
Now, we see that the how we can use induction becomes more clear.
</p>
</answer>
<solution>

<proof><p>
We are going to use mathematical induction.
</p>
<p>
<ul>
<li>
<p>
 <em>Base Case</em>: We see that for <m>n=1</m>, the statement is <q> <m>\displaystyle{\sum\limits_{k=1}^1 k^3=1=\left( \sum\limits_{k=1}^1 k \right)^2}</m> </q>. Thus, the statement is true for <m>n=1</m>.
</p>
</li>
<li>
<p>
<em>Inductive Step</em>: Let <m>m\geq 1</m> and assume that the statement is true for <m>n=m</m>, that is, assume that <m>\displaystyle{\sum\limits_{k=1}^m k^3=\left( \sum\limits_{k=1}^m k \right)^2}</m>. Then, <me>\sum\limits_{k=1}^{m+1} k^3=\sum\limits_{k=1}^m k^3+(m+1)^3=\left( \sum\limits_{k=1}^m k \right)^2+(m+1)^3.</me>
</p>
<p>
Moreover, we know that <m>\displaystyle{\sum\limits_{k=1}^m k}=\dfrac{m(m+1)}{2}</m>. Hence,
<me>\sum\limits_{k=1}^{m+1} k^3=\frac{m^2(m+1)^2}{4}+(m+1)^3= \frac{(m+1)^2(m^2+4m+1)}{4}=\frac{(m+1)^2(m+2)^2}{4}= \left( \sum\limits_{k=1}^{m+1} k \right)^2.</me>
</p></li>
</ul>
</p>
<p>
Therefore the statement is true for <m>n=m+1</m>, and hence, by induction, it is true for all <m>n\in\mathbb{N}</m>.
</p></proof>

</solution>
</exercise>
