<exercise>
<!-- source latex = 'sum of exponentials.tex' -->
<!-- converted on 08/11/2021 at 10:55 -->
<statement>
<p>
Let <m>n\in\mathbb{N}\cup\{0\}</m>. Show that <m>5</m> divides <m>2^{2n+1}+3^{2n+1}</m>.
</p>
</statement>

<!-- <hint></hint> -->

<answer>
<p>
We want to prove this statement by induction on <m>n</m>.
<ul>
<li>
<p>
 Base case: Take <m>n=0</m>. Then <m> 2^{2n+1}+3^{2n+1} =2+3=5, </m>, so the result holds.
</p></li>
<li>
<p>
 Inductive step: Assume that
<me> 5\mid \left(2^{2k+1}+3^{2k+1}\right). </me>
We want to show that
<me> 5\mid \left( 2^{2(k+1)+1}+3^{2(k+1)+1} \right). </me>
The assumption tells us that there is some <m>\ell\in\mathbb{Z}</m> such that
<me> 2^{2k+1}+3^{2k+1} = 5\ell. </me>
Note that
<me> 2^{2(k+1)+1}+3^{2(k+1)+1} =4\cdot2^{2k+1}+9\cdot 3^{2k+1}=4(2^{2k+1}+3^{2k+1})+5\cdot 3^{2k+1} </me>
and so by the inductive hypothesis
<me> 2^{2(k+1)+1}+3^{2(k+1)+1} =4\cdot 5\ell+5\cdot 3^{2k+1} =5(4\ell+3^{2k+1}). </me>
Therefore <m>2^{2(k+1)+1}+3^{2(k+1)+1}</m> is divisible by <m>5</m>.
</p></li>
<li>
<p>
 Another way to prove the inductive step is to consider the difference
<me> 2^{2(k+1)+1}+3^{2(k+1)+1}-(2^{2k+1}+3^{2k+1}) </me>
and show that it is divisible by <m>5</m>.
To this end, let's simplify that difference:
<md>
<mrow>
2^{2(k+1)+1}+3^{2(k+1)+1}-(2^{2k+1}+3^{2k+1})  \amp =3^{2(k+1)+1}-3^{2k+1}+2^{2(k+1)+1}-2^{2k+1}
</mrow><mrow>
 \amp =3^2\cdot 3^{2k+1}-3^{2k+1}+2^2\cdot 2^{2k+1}-2^{2k+1}
</mrow><mrow>
 \amp =8\cdot 3^{2k+1}+3\cdot2^{2k+1}
</mrow>
</md>
We want to rewrite this expression in terms of <m>2^{2k+1}+3^{2k+1}</m>, so that we can use the inductive hypothesis. We rewrite the expression above as
<me> 8\cdot 3^{2k+1}+3\cdot2^{2k+1} = 8\cdot (3^{2k+1}+2^{2k+1})-8\cdot 2^{2k+1}+3\cdot2^{2k+1} </me>
This is equal to
<me>  8\cdot (3^{2k+1}+2^{2k+1})-5\cdot2^{2k+1}</me>
which is divisibly by <m>5</m>, since the second term is divisible by <m>5</m>, and the first is by the inductive hypothesis.
</p>

</li>
</ul>
</p>
<p>
Now we can write the formal proof.
</p>
</answer>
<solution>

<proof>
<p>
Let <m>n\in\mathbb{N}</m>.
We proceed by induction on <m>n</m>. When <m>n=0</m>, we have
<me> 2^{2n+1}+3^{2n+1} =2+3=5, </me>
which is divisible by <m>5</m>. Now suppose that the result holds for <m>n=k</m>, so
<me> 5\mid \left( 2^{2k+1}+3^{2k+1} \right). </me>
Then there is some <m>\ell\in\mathbb{Z}</m> such that
<me> 2^{2k+1}+3^{2k+1} = 5\ell. </me>
Note that
<me> 2^{2(k+1)+1}+3^{2(k+1)+1} =4\cdot2^{2k+1}+9\cdot 3^{2k+1}=4(2^{2k+1}+3^{2k+1})+5\cdot 3^{2k+1}. </me>
Then by the inductive hypothesis
<me> 2^{2(k+1)+1}+3^{2(k+1)+1} =4\cdot 5\ell+5\cdot 3^{2k+1} =5(4\ell+3^{2k+1}) </me>
and so <m>5</m> divides <m>2^{2(k+1)+1}+3^{2(k+1)+1}</m>. Therefore, by induction, <m>5</m> divides <m>2^{2n+1}+3^{2n+1}</m> for all <m>n\in\mathbb{N}</m>.
</p>
</proof>

</solution>
</exercise>
