<exercise>
<!-- source latex = 'there is x and y and z such that x quare plus y square is equal to z to the 2n plus 1 question.tex' -->
<!-- converted on 12/08/2021 at 20:03 -->
<statement>
<p>
Let <m>n\in\mathbb N</m>. Prove by induction on <m>n</m>, that <m>\exists x,y,z\in \mathbb Z</m> such that <m>x\geq 2</m>, <m>y\geq 2</m>, and <m>z\geq 2</m> and satisfy <m>x^2+y^2=z^{2n+1}</m>.
</p>
</statement>

<hint>
<p>
How can we get from <m>z^{2n+1}</m> to <m>z^{2(n+1)+1}</m>?
</p>
</hint>

<solution>
<p>
The question wants us to use mathematical induction. However, we also see that this is not a standard induction question in the sense that for all <m>n\in\mathbb N</m>, we actually want to prove an existential statement, that is, the existence of <m>x,y</m>, and <m>z</m> satisfying <m>x^2+y^2=z^{2n+1}</m>. Let's see how we can do that in the proof.
</p>

<proof><p>
We are going to use mathematical induction.
</p>
<p>
<ul>
<li>
<p>
<em>Base Case</em>: We see that for <m>n=1</m>, the stament is  <q><m>\exists x,y,z\in \mathbb Z</m> such that <m>x\geq 2</m>, <m>y\geq 2</m>, and <m>z\geq 2</m> and satisfy <m>x^2+y^2=z^{3}</m></q>. We see that for <m>x=2</m>, <m>y=2</m>, and <m>z=2</m>, this statement is true.
</p>
</li>
<li>
<p>
<em>Inductive Step</em>: Let <m>k\geq 1</m>, and assume that the statement is true for <m>n=k</m>, that is, <m>\exists x,y,z\in \mathbb Z</m> such that <m>x\geq 2</m>, <m>y\geq 2</m>, and <m>z\geq 2</m> and satisfy <m>x^2+y^2=z^{2k+1}</m>. Then we see that if we multiply the equation by <m>z^2</m>, we get <m>(xz)^2+(yz)^2=z^{2k+3}=z^{2(k+1)+1}</m>. Moreover, we see that <m>(xz),(xy)\geq 2</m> since <m>x,z,y\geq 2</m>.
</p></li>
</ul>
</p>
<p>
Therefore the statement is true for <m>n=k+1</m>, and hence, by induction, it is true for all <m>n\in\mathbb{N}</m>.
</p>

</proof>

</solution>
</exercise>
